src/program_proof/tulip/program/backup/backup.v
@@ -1,9 +1,14 @@
 From Perennial.program_proof.tulip.program Require Import prelude.
-From Perennial.program_proof.tulip.invariance Require Import prepare unprepare.
+From Perennial.program_proof.tulip.invariance Require Import propose prepare unprepare.
+From Perennial.program_proof.tulip.program Require Import quorum.
 (* import for [local_gid_token] *)
 From Perennial.program_proof.tulip.program.txn Require Import res.
 (* for common definitions; TODO: factoring them out *)
 From Perennial.program_proof.tulip.program.gcoord Require Import gpreparer_repr.
+(* for [try_resign] related resources *)
+From Perennial.program_proof.tulip.program.gcoord Require Import gpreparer_try_resign.
+(* for [sum_no_overflow] *)
+From Perennial.program_proof Require Import std_proof.
 
 Inductive bgppphase :=
 | BGPPInquiring
@@ -14,6 +19,11 @@ Inductive bgppphase :=
 | BGPPCommitted
 | BGPPAborted
 | BGPPStopped.
+
+#[global]
+Instance bgppphase_eq_decision :
+  EqDecision bgppphase.
+Proof. solve_decision. Qed.
 
 Definition bgppphase_to_u64 phase :=
   match phase with
@@ -73,12 +83,12 @@ Proof. intros x y H. by destruct x, y. Defined.
 Section bgpp_repr.
   Context `{!heapGS Σ, !tulip_ghostG Σ}.
 
-  Definition safe_backup_gpreparer_phase γ ts gid rk phase : iProp Σ :=
+  Definition safe_backup_gpreparer_phase γ ts cid gid rk phase : iProp Σ :=
     match phase with
     | BGPPInquiring => True
-    | BGPPValidating => True
-    | BGPPPreparing =>
-        quorum_validated γ gid ts ∗ is_group_prepare_proposal γ gid ts rk true
+    | BGPPValidating =>
+        safe_proposal γ gid ts rk true ∗ quorum_voted γ gid ts rk cid
+    | BGPPPreparing => is_group_prepare_proposal γ gid ts rk true
     | BGPPUnpreparing => is_group_prepare_proposal γ gid ts rk false
     | BGPPPrepared =>
         quorum_prepared γ gid ts ∗ quorum_validated γ gid ts
@@ -88,8 +98,8 @@ Section bgpp_repr.
     end.
 
   #[global]
-  Instance safe_backup_gpreparer_phase_persistent γ ts gid rk phase :
-    Persistent (safe_backup_gpreparer_phase γ ts gid rk phase).
+  Instance safe_backup_gpreparer_phase_persistent γ ts cid gid rk phase :
+    Persistent (safe_backup_gpreparer_phase γ ts cid gid rk phase).
   Proof. destruct phase; apply _. Defined.
 
   Definition safe_backup_gpreparer_action γ ts gid rk action : iProp Σ :=
@@ -145,10 +155,20 @@ Section bgpp_repr.
       "#Hpwrs"     ∷ (if pwrsok then own_map pwrsP DfracDiscarded pwrs else True) ∗
       "#Hsafepwrs" ∷ (if pwrsok then safe_txn_pwrs γ gid ts pwrs else True).
 
-  Definition own_backup_gpreparer_pps (gpp : loc) : iProp Σ :=
-    ∃ (ppsP : loc) (pps : gmap u64 ppsl),
-      "HppsP" ∷ gpp ↦[BackupGroupPreparer :: "pps"] #ppsP ∗
-      "Hpps"  ∷ own_map ppsP (DfracOwn 1) pps.
+  Definition own_backup_gpreparer_pps
+    (gpp : loc) (pps : gmap u64 ppsl) rk ts cid gid γ : iProp Σ :=
+    ∃ (ppsP : loc) (blts : gmap u64 ballot),
+      let n := latest_before_quorum rk blts in
+      "HppsP"    ∷ gpp ↦[BackupGroupPreparer :: "pps"] #ppsP ∗
+      "Hpps"     ∷ own_map ppsP (DfracOwn 1) pps ∗
+      "#Hblts"   ∷ ([∗ map] rid ↦ blt ∈ blts, is_replica_ballot_lb γ gid rid ts blt) ∗
+      "#Hpsl"    ∷ ([∗ map] pp ∈ pps,
+                      is_group_prepare_proposal_if_classic γ gid ts (uint.nat pp.1) pp.2) ∗
+      "#Hvotes"  ∷ ([∗ set] rid ∈ dom pps, is_replica_backup_vote γ gid rid ts rk cid) ∗
+      "%Hdompps" ∷ ⌜dom pps ⊆ rids_all⌝ ∗
+      "%Hlen"    ∷ ⌜map_Forall (λ _ l, (rk = length l)%nat) blts⌝ ∗
+      "%Hblts"   ∷ ⌜map_Forall2 (λ k pp blt, latest_term blt = uint.nat pp.1 ∧
+                                             blt !! uint.nat pp.1 = Some (Accept pp.2)) pps blts⌝.
 
   Definition own_backup_gpreparer_vdm (gpp : loc) ts gid γ : iProp Σ :=
     ∃ (vdmP : loc) (vdm : gmap u64 bool),
@@ -157,40 +177,67 @@ Section bgpp_repr.
       "#Hvds"   ∷ validation_responses γ ts gid vdm ∗
       "%Hvincl" ∷ ⌜dom vdm ⊆ rids_all⌝.
 
-  Definition prepare_responses γ ts gid phase (srespm : gmap u64 bool) : iProp Σ :=
+  Definition prepare_responses γ rk ts gid phase (srespm : gmap u64 bool) : iProp Σ :=
     match phase with
     | BGPPPreparing =>
-        ([∗ set] rid ∈ dom srespm, is_replica_pdec_at_rank γ gid rid ts 1%nat true)
+        ([∗ set] rid ∈ dom srespm, is_replica_pdec_at_rank γ gid rid ts rk true)
     | BGPPUnpreparing =>
-        ([∗ set] rid ∈ dom srespm, is_replica_pdec_at_rank γ gid rid ts 1%nat false)
+        ([∗ set] rid ∈ dom srespm, is_replica_pdec_at_rank γ gid rid ts rk false)
     | _ => True
     end.
 
   #[global]
-  Instance prepare_responses_persistent γ ts gid phase srespm :
-    Persistent (prepare_responses γ ts gid phase srespm).
+  Instance prepare_responses_persistent γ rk ts gid phase srespm :
+    Persistent (prepare_responses γ rk ts gid phase srespm).
   Proof. destruct phase; apply _. Defined.
 
   Definition own_backup_gpreparer_srespm
-    (gpp : loc) (phase : bgppphase) ts gid γ : iProp Σ :=
+    (gpp : loc) (phase : bgppphase) rk ts gid γ : iProp Σ :=
     ∃ (srespmP : loc) (srespm : gmap u64 bool),
       "HsrespmP" ∷ gpp ↦[BackupGroupPreparer :: "srespm"] #srespmP ∗
       "Hsrespm"  ∷ own_map srespmP (DfracOwn 1) srespm ∗
-      "#Hpreps"  ∷ prepare_responses γ ts gid phase srespm ∗
+      "#Hpreps"  ∷ prepare_responses γ rk ts gid phase srespm ∗
       "%Hsincl"  ∷ ⌜dom srespm ⊆ rids_all⌝.
 
-  Definition own_backup_gpreparer_with_phase gpp phase rk ts gid γ : iProp Σ :=
-    "Hnrps"   ∷ own_backup_gpreparer_nrps gpp ∗
-    "Hphase"  ∷ own_backup_gpreparer_phase gpp phase ∗
-    "Hpwrs"   ∷ own_backup_gpreparer_pwrs gpp ts gid γ ∗
-    "Hpps"    ∷ own_backup_gpreparer_pps gpp ∗
-    "Hvdm"    ∷ own_backup_gpreparer_vdm gpp ts gid γ ∗
-    "Hsrespm" ∷ own_backup_gpreparer_srespm gpp phase ts gid γ ∗
-    "#Hsafe"  ∷ safe_backup_gpreparer_phase γ ts gid rk phase.
+  Definition accepting_phase phase :=
+    match phase with
+    | BGPPPreparing => True
+    | BGPPUnpreparing => True
+    | _ => False
+    end.
 
-  Definition own_backup_gpreparer gpp rk ts gid γ : iProp Σ :=
+  Lemma own_backup_gpreparer_srespm_non_accepting_phase gpp phase phase' rk ts gid γ :
+    not (accepting_phase phase')  ->
+    own_backup_gpreparer_srespm gpp phase rk ts gid γ -∗
+    own_backup_gpreparer_srespm gpp phase' rk ts gid γ.
+  Proof.
+    iIntros (Hna) "Hgpp".
+    iNamed "Hgpp".
+    iFrame "∗ %".
+    by destruct phase'.
+  Qed.
+
+  Definition own_replica_backup_token_cond phase rk ts cid gid γ : iProp Σ :=
+    match phase with
+    | BGPPInquiring => own_replica_backup_token γ cid.1 cid.2 ts rk gid
+    | BGPPValidating => own_replica_backup_token γ cid.1 cid.2 ts rk gid
+    | _ => True
+    end.
+
+  Definition own_backup_gpreparer_with_phase gpp phase rk ts cid gid γ : iProp Σ :=
+    ∃ (pps : gmap u64 ppsl),
+      "Hnrps"   ∷ own_backup_gpreparer_nrps gpp ∗
+      "Hphase"  ∷ own_backup_gpreparer_phase gpp phase ∗
+      "Hpwrs"   ∷ own_backup_gpreparer_pwrs gpp ts gid γ ∗
+      "Hpps"    ∷ own_backup_gpreparer_pps gpp pps rk ts cid gid γ ∗
+      "Hvdm"    ∷ own_backup_gpreparer_vdm gpp ts gid γ ∗
+      "Hsrespm" ∷ own_backup_gpreparer_srespm gpp phase rk ts gid γ ∗
+      "Htoken"  ∷ own_replica_backup_token_cond phase rk ts cid gid γ ∗
+      "#Hsafe"  ∷ safe_backup_gpreparer_phase γ ts cid gid rk phase.
+
+  Definition own_backup_gpreparer gpp rk ts cid gid γ : iProp Σ :=
     ∃ (phase : bgppphase),
-      "Hgpp" ∷ own_backup_gpreparer_with_phase gpp phase rk ts gid γ.
+      "Hgpp" ∷ own_backup_gpreparer_with_phase gpp phase rk ts cid gid γ.
 
 End bgpp_repr.
 
@@ -213,10 +260,10 @@ Section bgcoord_repr.
   (*@     // Connections to replicas.                                         @*)
   (*@     conns     map[uint64]grove_ffi.Connection                           @*)
   (*@ }                                                                       @*)
-  Definition own_backup_gcoord_gpreparer gcoord rk ts gid γ : iProp Σ :=
+  Definition own_backup_gcoord_gpreparer gcoord rk ts cid gid γ : iProp Σ :=
     ∃ (gppP : loc),
       "HgppP" ∷ gcoord ↦[BackupGroupCoordinator :: "gpp"] #gppP ∗
-      "Hgpp"  ∷ own_backup_gpreparer gppP rk ts gid γ.
+      "Hgpp"  ∷ own_backup_gpreparer gppP rk ts cid gid γ.
 
   Definition own_backup_gcoord_comm gcoord (addrm : gmap u64 chan) gid γ : iProp Σ :=
     ∃ (connsP : loc) (conns : gmap u64 (chan * chan)),
@@ -226,8 +273,8 @@ Section bgcoord_repr.
       "#Htrmls" ∷ ([∗ map] x ∈ conns, is_terminal γ gid x.1) ∗
       "%Haddrm" ∷ ⌜map_Forall (λ rid x, addrm !! rid = Some x.2) conns⌝.
 
-  Definition own_backup_gcoord gcoord addrm rk ts gid γ : iProp Σ :=
-    "Hgpp"  ∷ own_backup_gcoord_gpreparer gcoord rk ts gid γ ∗
+  Definition own_backup_gcoord gcoord addrm rk ts cid gid γ : iProp Σ :=
+    "Hgpp"  ∷ own_backup_gcoord_gpreparer gcoord rk ts cid gid γ ∗
     "Hcomm" ∷ own_backup_gcoord_comm gcoord addrm gid γ.
 
   Definition is_backup_gcoord_addrm gcoord (addrm : gmap u64 chan) : iProp Σ :=
@@ -243,11 +290,12 @@ Section bgcoord_repr.
       "%Hnodup"    ∷ ⌜NoDup rps⌝.
 
   Definition is_backup_gcoord_with_addrm gcoord (addrm : gmap u64 chan) rk ts gid γ : iProp Σ :=
-    ∃ (muP : loc) (cvP : loc),
+    ∃ (muP : loc) (cvP : loc) (cid : coordid),
       "#HmuP"    ∷ readonly (gcoord ↦[BackupGroupCoordinator :: "mu"] #muP) ∗
-      "#Hlock"   ∷ is_lock tulipNS #muP (own_backup_gcoord gcoord addrm rk ts gid γ) ∗
+      "#Hlock"   ∷ is_lock tulipNS #muP (own_backup_gcoord gcoord addrm rk ts cid gid γ) ∗
       "#HcvP"    ∷ readonly (gcoord ↦[BackupGroupCoordinator :: "cv"] #cvP) ∗
       "#Hcv"     ∷ is_cond cvP #muP ∗
+      "#HcidP"   ∷ readonly (gcoord ↦[BackupGroupCoordinator :: "cid"] (coordid_to_val cid)) ∗
       "#Hinv"    ∷ know_tulip_inv γ ∗
       "#Hinvnet" ∷ know_tulip_network_inv γ gid addrm ∗
       "#Haddrm"  ∷ is_backup_gcoord_addrm gcoord addrm ∗
@@ -342,11 +390,11 @@ Section bgpreparer.
     }
   Qed.
 
-  Theorem wp_BackupGroupPreparer__ready_external (gpp : loc) phase rk ts gid γ :
-    {{{ own_backup_gpreparer_with_phase gpp phase rk ts gid γ }}}
+  Theorem wp_BackupGroupPreparer__ready_external (gpp : loc) phase rk ts cid gid γ :
+    {{{ own_backup_gpreparer_with_phase gpp phase rk ts cid gid γ }}}
       BackupGroupPreparer__ready #gpp
     {{{ RET #(bool_decide (bgpp_ready phase)); 
-        own_backup_gpreparer_with_phase gpp phase rk ts gid γ
+        own_backup_gpreparer_with_phase gpp phase rk ts cid gid γ
     }}}.
   Proof.
     iIntros (Φ) "Hgpp HΦ".
@@ -357,12 +405,12 @@ Section bgpreparer.
     by iFrame "∗ #".
   Qed.
 
-  Theorem wp_BackupGroupPreparer__getPhase (gpp : loc) phase rk ts gid γ :
-    {{{ own_backup_gpreparer_with_phase gpp phase rk ts gid γ }}}
+  Theorem wp_BackupGroupPreparer__getPhase (gpp : loc) phase rk ts cid gid γ :
+    {{{ own_backup_gpreparer_with_phase gpp phase rk ts cid gid γ }}}
       BackupGroupPreparer__getPhase #gpp
     {{{ RET #(bgppphase_to_u64 phase); 
-        own_backup_gpreparer_with_phase gpp phase rk ts gid γ ∗
-        safe_backup_gpreparer_phase γ ts gid rk phase
+        own_backup_gpreparer_with_phase gpp phase rk ts cid gid γ ∗
+        safe_backup_gpreparer_phase γ ts cid gid rk phase
     }}}.
   Proof.
     iIntros (Φ) "Hgpp HΦ".
@@ -379,10 +427,10 @@ Section bgpreparer.
   Qed.
 
   (* A weak spec since its use is not related to safety *)
-  Theorem wp_BackupGroupPreparer__finalized gpp rk ts gid γ :
-    {{{ own_backup_gpreparer gpp rk ts gid γ }}}
+  Theorem wp_BackupGroupPreparer__finalized gpp rk ts cid gid γ :
+    {{{ own_backup_gpreparer gpp rk ts cid gid γ }}}
       BackupGroupPreparer__finalized #gpp
-    {{{ (finalized : bool), RET #finalized; own_backup_gpreparer gpp rk ts gid γ }}}.
+    {{{ (finalized : bool), RET #finalized; own_backup_gpreparer gpp rk ts cid gid γ }}}.
   Proof.
     iIntros (Φ) "Hgpp HΦ".
     wp_rec.
@@ -397,87 +445,179 @@ Section bgpreparer.
     by iFrame "∗ # %".
   Qed.
 
-  Theorem wp_BackupGroupPreparer__action (gpp : loc) (rid : u64) rk ts gid γ :
-    {{{ own_backup_gpreparer gpp rk ts gid γ }}}
+  (* Rather weak spec as it's used only in a performance optimization. *)
+  Theorem wp_BackupGroupPreparer__inquired (gpp : loc) (rid : u64) pps rk ts cid gid γ :
+    {{{ own_backup_gpreparer_pps gpp pps rk ts cid gid γ }}}
+      BackupGroupPreparer__inquired #gpp #rid
+    {{{ (inquired : bool), RET #inquired; own_backup_gpreparer_pps gpp pps rk ts cid gid γ }}}.
+  Proof.
+    (*@ func (gpp *BackupGroupPreparer) inquired(rid uint64) bool {             @*)
+    (*@     _, inquired := gpp.pps[rid]                                         @*)
+    (*@     return inquired                                                     @*)
+    (*@ }                                                                       @*)
+  Admitted.
+
+  (* Rather weak spec as it's used only in a performance optimization. *)
+  Theorem wp_BackupGroupPreparer__validated (gpp : loc) (rid : u64) ts gid γ :
+    {{{ own_backup_gpreparer_vdm gpp ts gid γ }}}
+      BackupGroupPreparer__validated #gpp #rid
+    {{{ (validated : bool), RET #validated; own_backup_gpreparer_vdm gpp ts gid γ }}}.
+  Proof.
+    (*@ func (gpp *BackupGroupPreparer) validated(rid uint64) bool {            @*)
+    (*@     _, validated := gpp.vdm[rid]                                        @*)
+    (*@     return validated                                                    @*)
+    (*@ }                                                                       @*)
+  Admitted.
+
+  (* Rather weak spec as it's used only in a performance optimization. *)
+  Theorem wp_BackupGroupPreparer__accepted (gpp : loc) (rid : u64) phase rk ts gid γ :
+    {{{ own_backup_gpreparer_srespm gpp phase rk ts gid γ }}}
+      BackupGroupPreparer__accepted #gpp #rid
+    {{{ (accepted : bool), RET #accepted; own_backup_gpreparer_srespm gpp phase rk ts gid γ }}}.
+  Proof.
+    (*@ func (gpp *BackupGroupPreparer) accepted(rid uint64) bool {             @*)
+    (*@     _, accepted := gpp.srespm[rid]                                      @*)
+    (*@     return accepted                                                     @*)
+    (*@ }                                                                       @*)
+  Admitted.
+
+  Theorem wp_BackupGroupPreparer__action (gpp : loc) (rid : u64) rk ts cid gid γ :
+    {{{ own_backup_gpreparer gpp rk ts cid gid γ }}}
       BackupGroupPreparer__action #gpp #rid
     {{{ (action : bgppaction), RET #(bgppaction_to_u64 action); 
-        own_backup_gpreparer gpp rk ts gid γ ∗
+        own_backup_gpreparer gpp rk ts cid gid γ ∗
         safe_backup_gpreparer_action γ ts gid rk action
     }}}.
   Proof.
+    iIntros (Φ) "Hgpp HΦ".
+    wp_rec.
+
     (*@ func (gpp *BackupGroupPreparer) action(rid uint64) uint64 {             @*)
+    (*@     phase := gpp.getPhase()                                             @*)
+    (*@                                                                         @*)
+    iNamed "Hgpp".
+    wp_apply (wp_BackupGroupPreparer__getPhase with "Hgpp").
+    iIntros "[Hgpp _]".
+    wp_pures.
+    iNamed "Hgpp".
+
     (*@     // Inquire the transaction status on replica @rid.                  @*)
-    (*@     if gpp.phase == BGPP_INQUIRING {                                    @*)
+    (*@     if phase == BGPP_INQUIRING {                                        @*)
     (*@         // Check if the inquire response (i.e., latest proposal + validation @*)
     (*@         // status) for replica @rid is available.                       @*)
-    (*@         _, inquired := gpp.pps[rid]                                     @*)
+    (*@         inquired := gpp.inquired(rid)                                   @*)
     (*@         if !inquired {                                                  @*)
     (*@             // Have not received the inquire response.                  @*)
     (*@             return BGPP_INQUIRE                                         @*)
     (*@         }                                                               @*)
-    (*@                                                                         @*)
     (*@         return BGPP_REFRESH                                             @*)
     (*@     }                                                                   @*)
     (*@                                                                         @*)
+    case_bool_decide as Hinquiring; wp_pures.
+    { wp_apply (wp_BackupGroupPreparer__inquired with "Hpps").
+      iIntros (inquired) "Hpps".
+      wp_pures.
+      destruct inquired; wp_pures; last first.
+      { iApply ("HΦ" $! BGPPInquire). by iFrame. }
+      iApply ("HΦ" $! BGPPRefresh). by iFrame.
+    }
+
     (*@     // Validate the transaction.                                        @*)
-    (*@     if gpp.phase == BGPP_VALIDATING {                                   @*)
+    (*@     if phase == BGPP_VALIDATING {                                       @*)
     (*@         // Check if the inquire response (i.e., latest proposal + validation @*)
     (*@         // status) for replica @rid is available.                       @*)
-    (*@         _, inquired := gpp.pps[rid]                                     @*)
+    (*@         inquired := gpp.inquired(rid)                                   @*)
     (*@         if !inquired {                                                  @*)
     (*@             // Have not received inquire response.                      @*)
     (*@             return BGPP_INQUIRE                                         @*)
     (*@         }                                                               @*)
-    (*@                                                                         @*)
     (*@         // The inquire response is available. Now check if the transaction has @*)
     (*@         // been validated on replica @rid.                              @*)
-    (*@         _, validated := gpp.vdm[rid]                                    @*)
+    (*@         validated := gpp.validated(rid)                                 @*)
     (*@         if !validated {                                                 @*)
     (*@             return BGPP_VALIDATE                                        @*)
     (*@         }                                                               @*)
-    (*@                                                                         @*)
     (*@         return BGPP_REFRESH                                             @*)
     (*@     }                                                                   @*)
     (*@                                                                         @*)
+    case_bool_decide as Hvalidating; wp_pures.
+    { wp_apply (wp_BackupGroupPreparer__inquired with "Hpps").
+      iIntros (inquired) "Hpps".
+      wp_pures.
+      destruct inquired; wp_pures; last first.
+      { iApply ("HΦ" $! BGPPInquire). by iFrame. }
+      wp_apply (wp_BackupGroupPreparer__validated with "Hvdm").
+      iIntros (validated) "Hvdm".
+      wp_pures.
+      destruct validated; wp_pures; last first.
+      { iApply ("HΦ" $! BGPPValidate). by iFrame. }
+      iApply ("HΦ" $! BGPPRefresh). by iFrame.
+    }
+
     (*@     // Prepare the transaction.                                         @*)
-    (*@     if gpp.phase == BGPP_PREPARING {                                    @*)
-    (*@         _, prepared := gpp.srespm[rid]                                  @*)
+    (*@     if phase == BGPP_PREPARING {                                        @*)
+    (*@         prepared := gpp.accepted(rid)                                   @*)
     (*@         if !prepared {                                                  @*)
     (*@             return BGPP_PREPARE                                         @*)
     (*@         }                                                               @*)
     (*@         return BGPP_REFRESH                                             @*)
     (*@     }                                                                   @*)
     (*@                                                                         @*)
+    case_bool_decide as Hpreparing; wp_pures.
+    { wp_apply (wp_BackupGroupPreparer__accepted with "Hsrespm").
+      iIntros (prepared) "Hsrespm".
+      wp_pures.
+      destruct prepared; wp_pures; last first.
+      { iApply ("HΦ" $! BGPPPrepare).
+        destruct phase; try done.
+        by iFrame "∗ #".
+      }
+      iApply ("HΦ" $! BGPPRefresh). by iFrame.
+    }
+
     (*@     // Unprepare the transaction.                                       @*)
-    (*@     if gpp.phase == BGPP_UNPREPARING {                                  @*)
-    (*@         _, unprepared := gpp.srespm[rid]                                @*)
+    (*@     if phase == BGPP_UNPREPARING {                                      @*)
+    (*@         unprepared := gpp.accepted(rid)                                 @*)
     (*@         if !unprepared {                                                @*)
     (*@             return BGPP_UNPREPARE                                       @*)
     (*@         }                                                               @*)
     (*@         return BGPP_REFRESH                                             @*)
     (*@     }                                                                   @*)
     (*@                                                                         @*)
+    case_bool_decide as Hunpreparing; wp_pures.
+    { wp_apply (wp_BackupGroupPreparer__accepted with "Hsrespm").
+      iIntros (unprepared) "Hsrespm".
+      wp_pures.
+      destruct unprepared; wp_pures; last first.
+      { iApply ("HΦ" $! BGPPUnprepare).
+        destruct phase; try done.
+        by iFrame "∗ #".
+      }
+      iApply ("HΦ" $! BGPPRefresh). by iFrame.
+    }
+
     (*@     return BGPP_REFRESH                                                 @*)
     (*@ }                                                                       @*)
-  Admitted.
+    iApply ("HΦ" $! BGPPRefresh). by iFrame.
+  Qed.
 
-  Theorem wp_BackupGroupPreparer__getPwrs (gpp : loc) rk ts gid γ :
-    {{{ own_backup_gpreparer gpp rk ts gid γ }}}
+  Theorem wp_BackupGroupPreparer__getPwrs (gpp : loc) ts gid γ :
+    {{{ own_backup_gpreparer_pwrs gpp ts gid γ }}}
       BackupGroupPreparer__getPwrs #gpp
     {{{ (pwrsP : loc) (pwrsok : bool), RET (#pwrsP, #pwrsok);
-        own_backup_gpreparer gpp rk ts gid γ ∗
+        own_backup_gpreparer_pwrs gpp ts gid γ ∗
         if pwrsok
         then ∃ pwrs, own_map pwrsP DfracDiscarded pwrs ∗ safe_txn_pwrs γ gid ts pwrs
         else True
     }}}.
   Proof.
-    iIntros (Φ) "Hgpp HΦ".
+    iIntros (Φ) "Hpwrs HΦ".
     wp_rec.
 
     (*@ func (gpp *BackupGroupPreparer) getPwrs() (tulip.KVMap, bool) {         @*)
     (*@     return gpp.pwrs, gpp.pwrsok                                         @*)
     (*@ }                                                                       @*)
-    do 2 iNamed "Hgpp". iNamed "Hpwrs".
+    iNamed "Hpwrs".
     do 2 wp_loadField.
     wp_pures.
     iModIntro.
@@ -485,6 +625,1533 @@ Section bgpreparer.
     iFrame "∗ # %".
     destruct pwrsok; last done.
     by eauto.
+  Qed.
+
+  Theorem wp_BackupGroupPreparer__getPwrs_external (gpp : loc) rk ts cid gid γ :
+    {{{ own_backup_gpreparer gpp rk ts cid gid γ }}}
+      BackupGroupPreparer__getPwrs #gpp
+    {{{ (pwrsP : loc) (pwrsok : bool), RET (#pwrsP, #pwrsok);
+        own_backup_gpreparer gpp rk ts cid gid γ ∗
+        if pwrsok
+        then ∃ pwrs, own_map pwrsP DfracDiscarded pwrs ∗ safe_txn_pwrs γ gid ts pwrs
+        else True
+    }}}.
+  Proof.
+    iIntros (Φ) "Hgpp HΦ".
+    do 2 iNamed "Hgpp".
+    wp_apply (wp_BackupGroupPreparer__getPwrs with "Hpwrs").
+    iIntros (pwrsP pwrsok) "[Hpwrs Hm]".
+    iApply "HΦ".
+    by iFrame "∗ # %".
+  Qed.
+
+  Theorem wp_BackupGroupPreparer__tryResign (gpp : loc) (res : rpres) phase rk ts cid gid γ :
+    try_resign_requirement γ ts res -∗
+    {{{ own_backup_gpreparer_with_phase gpp phase rk ts cid gid γ }}}
+      BackupGroupPreparer__tryResign #gpp #(rpres_to_u64 res)
+    {{{ (resigned : bool) (phase' : bgppphase), RET #resigned;
+        own_backup_gpreparer_with_phase gpp phase' rk ts cid gid γ ∗
+        ⌜(if resigned then True else not_finalizing_rpres res)⌝ ∗
+        ⌜resigned = bool_decide (bgpp_ready phase')⌝
+    }}}.
+  Proof.
+    iIntros "#Hreq" (Φ) "!> Hgpp HΦ".
+    wp_rec.
+
+    (*@ func (gpp *BackupGroupPreparer) tryResign(res uint64) bool {            @*)
+    (*@     if gpp.ready() {                                                    @*)
+    (*@         return true                                                     @*)
+    (*@     }                                                                   @*)
+    (*@                                                                         @*)
+    wp_apply (wp_BackupGroupPreparer__ready_external with "Hgpp").
+    iIntros "Hgpp".
+    case_bool_decide as Hready; wp_pures.
+    { iApply "HΦ".
+      case_bool_decide; last done.
+      by iFrame.
+    }
+    iNamed "Hgpp". iNamed "Hphase".
+                
+    (*@     if res == tulip.REPLICA_COMMITTED_TXN {                             @*)
+    (*@         gpp.phase = BGPP_COMMITTED                                      @*)
+    (*@         return true                                                     @*)
+    (*@     }                                                                   @*)
+    (*@                                                                         @*)
+    case_bool_decide as Hcommitted; wp_pures.
+    { wp_storeField.
+      iModIntro.
+      iApply "HΦ".
+      destruct res; try done. simpl.
+      iDestruct (own_backup_gpreparer_srespm_non_accepting_phase _ _ BGPPCommitted with "Hsrespm")
+        as "Hsrespm".
+      { intros []. }
+      by iFrame "∗ #".
+    }
+
+    (*@     if res == tulip.REPLICA_ABORTED_TXN {                               @*)
+    (*@         gpp.phase = BGPP_ABORTED                                        @*)
+    (*@         return true                                                     @*)
+    (*@     }                                                                   @*)
+    (*@                                                                         @*)
+    case_bool_decide as Haborted; wp_pures.
+    { wp_storeField.
+      iModIntro.
+      iApply "HΦ".
+      destruct res; try done. simpl.
+      iDestruct (own_backup_gpreparer_srespm_non_accepting_phase _ _ BGPPAborted with "Hsrespm")
+        as "Hsrespm".
+      { intros []. }
+      by iFrame "∗ #".
+    }
+
+    (*@     if res == tulip.REPLICA_STALE_COORDINATOR {                         @*)
+    (*@         gpp.phase = BGPP_STOPPED                                        @*)
+    (*@         return true                                                     @*)
+    (*@     }                                                                   @*)
+    (*@                                                                         @*)
+    case_bool_decide as Hstopped; wp_pures.
+    { wp_storeField.
+      iModIntro.
+      iApply "HΦ".
+      destruct res; try done. simpl.
+      iDestruct (own_backup_gpreparer_srespm_non_accepting_phase _ _ BGPPStopped with "Hsrespm")
+        as "Hsrespm".
+      { intros []. }
+      by iFrame.
+    }
+
+    (*@     return false                                                        @*)
+    (*@ }                                                                       @*)
+    iApply ("HΦ" $! false phase).
+    case_bool_decide; first done.
+    iFrame "∗ # %".
+    iPureIntro.
+    by destruct res.
+  Qed.
+
+  Theorem wp_BackupGroupPreparer__in (gpp : loc) (phase phasecur : bgppphase) rk ts cid gid γ :
+    {{{ own_backup_gpreparer_with_phase gpp phasecur rk ts cid gid γ }}}
+      BackupGroupPreparer__in #gpp #(bgppphase_to_u64 phase)
+    {{{ RET #(bool_decide (phasecur = phase)); 
+        own_backup_gpreparer_with_phase gpp phasecur rk ts cid gid γ
+    }}}.
+  Proof.
+    iIntros (Φ) "Hgpp HΦ".
+    wp_rec.
+
+    (*@ func (gpp *BackupGroupPreparer) in(phase uint64) bool {                 @*)
+    (*@     return gpp.phase == phase                                           @*)
+    (*@ }                                                                       @*)
+    iNamed "Hgpp". iNamed "Hphase".
+    wp_loadField. wp_pures.
+    rewrite -Hphase.
+    case_bool_decide as Hcase.
+    { rewrite Hcase bool_decide_eq_true_2; last done.
+      iApply "HΦ".
+      by iFrame "∗ # %".
+    }
+    { rewrite bool_decide_eq_false_2; last first.
+      { by destruct phasecur, phase. }
+      iApply "HΦ".
+      by iFrame "∗ # %".
+    }
+  Qed.
+
+  Theorem wp_BackupGroupPreparer__collectProposal
+    (gpp : loc) (rid : u64) (pp : ppsl) pps rk ts cid gid γ :
+    rid ∈ rids_all ->
+    is_replica_backup_vote γ gid rid ts rk cid -∗
+    latest_proposal_replica γ gid rid ts rk (uint.nat pp.1) pp.2 -∗
+    {{{ own_backup_gpreparer_pps gpp pps rk ts cid gid γ }}}
+      BackupGroupPreparer__collectProposal #gpp #rid (ppsl_to_val pp)
+    {{{ RET #(); own_backup_gpreparer_pps gpp (<[rid := pp]> pps) rk ts cid gid γ }}}.
+  Proof.
+    iIntros (Hrid) "#Hvote #Hlatest".
+    iIntros (Φ) "!> Hpps HΦ".
+    wp_rec.
+
+    (*@ func (gpp *BackupGroupPreparer) collectProposal(rid uint64, pp tulip.PrepareProposal) { @*)
+    (*@     gpp.pps[rid] = pp                                                   @*)
+    (*@ }                                                                       @*)
+    iNamed "Hpps".
+    wp_loadField.
+    wp_apply (wp_MapInsert with "Hpps"); first done.
+    iIntros "Hpps".
+    wp_pures.
+    iModIntro.
+    iApply "HΦ".
+    iNamed "Hlatest".
+    iDestruct (big_sepM_insert_2 with "[] Hblts") as "Hblts'".
+    { by iFrame "Hlb". }
+    iClear "Hblts".
+    iFrame "∗ # %".
+    iSplit.
+    { by iApply big_sepM_insert_2. }
+    iSplit.
+    { rewrite dom_insert_L.
+      by iApply big_sepS_insert_2.
+    }
+    iPureIntro.
+    split.
+    { rewrite dom_insert_L. clear -Hrid Hdompps. set_solver. }
+    split.
+    { by apply map_Forall_insert_2. }
+    { by apply map_Forall2_insert_2. }
+  Qed.
+
+  Theorem wp_BackupGroupPreparer__collectProposal_weak
+    (gpp : loc) (rid : u64) (pp : ppsl) pps rk ts cid gid γ :
+    rid ∈ rids_all ->
+    is_replica_backup_vote γ gid rid ts rk cid -∗
+    latest_proposal_replica γ gid rid ts rk (uint.nat pp.1) pp.2 -∗
+    {{{ own_backup_gpreparer_pps gpp pps rk ts cid gid γ }}}
+      BackupGroupPreparer__collectProposal #gpp #rid (ppsl_to_val pp)
+    {{{ (pps' : gmap u64 ppsl), RET #(); 
+        own_backup_gpreparer_pps gpp pps' rk ts cid gid γ
+    }}}.
+  Proof.
+    iIntros (Hrid) "#Hvote #Hlatest".
+    iIntros (Φ) "!> Hpps HΦ".
+    by wp_apply (wp_BackupGroupPreparer__collectProposal with "Hvote Hlatest Hpps").
+  Qed.
+
+  Theorem wp_BackupGroupPreparer__setPwrs (gpp : loc) (pwrsP : loc) (pwrs : dbmap) ts gid γ :
+    own_map pwrsP DfracDiscarded pwrs -∗
+    safe_txn_pwrs γ gid ts pwrs -∗
+    {{{ own_backup_gpreparer_pwrs gpp ts gid γ }}}
+      BackupGroupPreparer__setPwrs #gpp #pwrsP
+    {{{ RET #(); own_backup_gpreparer_pwrs gpp ts gid γ }}}.
+  Proof.
+    iIntros "#Hm #Hsafe" (Φ) "!> Hpwrs HΦ".
+    wp_rec.
+
+    (*@ func (gpp *BackupGroupPreparer) setPwrs(pwrs tulip.KVMap) {             @*)
+    (*@     gpp.pwrsok = true                                                   @*)
+    (*@     gpp.pwrs = pwrs                                                     @*)
+    (*@ }                                                                       @*)
+    iNamed "Hpwrs".
+    do 2 wp_storeField.
+    iApply "HΦ".
+    by iFrame "∗ #".
+  Qed.
+
+  Theorem wp_BackupGroupPreparer__validate (gpp : loc) (rid : u64) ts gid γ :
+    rid ∈ rids_all ->
+    is_replica_validated_ts γ gid rid ts -∗
+    {{{ own_backup_gpreparer_vdm gpp ts gid γ }}}
+      BackupGroupPreparer__validate #gpp #rid
+    {{{ RET #(); own_backup_gpreparer_vdm gpp ts gid γ }}}.
+  Proof.
+    iIntros (Hrid) "#Hvd".
+    iIntros (Φ) "!> Hvdm HΦ".
+    wp_rec.
+
+    (*@ func (gpp *BackupGroupPreparer) validate(rid uint64) {                  @*)
+    (*@     gpp.vdm[rid] = true                                                 @*)
+    (*@ }                                                                       @*)
+    iNamed "Hvdm".
+    wp_loadField.
+    wp_apply (wp_MapInsert with "Hvdm"); first done.
+    iIntros "Hvdm".
+    wp_pures.
+    iModIntro.
+    iApply "HΦ".
+    iFrame "∗ # %".
+    iSplit.
+    { rewrite /validation_responses dom_insert_L.
+      by iApply big_sepS_insert_2.
+    }
+    iPureIntro.
+    rewrite dom_insert_L. set_solver.
+  Qed.
+
+  Theorem wp_BackupGroupPreparer__tryValidate
+    (gpp : loc) (rid : u64) (vd : bool) (pwrsP : loc) (pwrs : dbmap) ts gid γ :
+    rid ∈ rids_all ->
+    (if vd then own_map pwrsP DfracDiscarded pwrs else True) -∗
+    (if vd then safe_txn_pwrs γ gid ts pwrs else True) -∗
+    (if vd then is_replica_validated_ts γ gid rid ts else True) -∗
+    {{{ own_backup_gpreparer_pwrs gpp ts gid γ ∗ own_backup_gpreparer_vdm gpp ts gid γ }}}
+      BackupGroupPreparer__tryValidate #gpp #rid #vd #pwrsP
+    {{{ RET #();
+        own_backup_gpreparer_pwrs gpp ts gid γ ∗ own_backup_gpreparer_vdm gpp ts gid γ
+    }}}.
+  Proof.
+    iIntros (Hrid) "#Hm #Hsafepwrs #Hvd".
+    iIntros (Φ) "!> [Hpwrs Hvdm] HΦ".
+    wp_rec.
+
+    (*@ func (gpp *BackupGroupPreparer) tryValidate(rid uint64, vd bool, pwrs tulip.KVMap) { @*)
+    (*@     if vd {                                                             @*)
+    (*@         gpp.setPwrs(pwrs)                                               @*)
+    (*@         gpp.validate(rid)                                               @*)
+    (*@     }                                                                   @*)
+    (*@ }                                                                       @*)
+    wp_pures.
+    destruct vd; wp_pures.
+    { wp_apply (wp_BackupGroupPreparer__setPwrs with "Hm Hsafepwrs Hpwrs").
+      iIntros "Hpwrs".
+      wp_apply (wp_BackupGroupPreparer__validate with "Hvd Hvdm").
+      { apply Hrid. }
+      iIntros "Hvdm".
+      wp_pures.
+      iApply "HΦ".
+      by iFrame.
+    }
+    iApply "HΦ".
+    by iFrame.
+  Qed.
+
+  Theorem wp_BackupGroupPreparer__countProposals (gpp : loc) pps rk ts cid gid γ :
+    {{{ own_backup_gpreparer_pps gpp pps rk ts cid gid γ }}}
+      BackupGroupPreparer__countProposals #gpp
+    {{{ (n : u64), RET #n; 
+        own_backup_gpreparer_pps gpp pps rk ts cid gid γ ∗
+        ⌜uint.nat n = size pps⌝
+    }}}.
+  Proof.
+    iIntros (Φ) "Hpps HΦ".
+    wp_rec.
+
+    (*@ func (gpp *BackupGroupPreparer) countProposals() uint64 {               @*)
+    (*@     return uint64(len(gpp.pps))                                         @*)
+    (*@ }                                                                       @*)
+    iNamed "Hpps".
+    wp_loadField.
+    wp_apply (wp_MapLen with "Hpps").
+    iIntros "[%Hsz Hpps]".
+    iApply "HΦ".
+    iFrame "∗ # %".
+    word.
+  Qed.
+
+  Theorem wp_BackupGroupPreparer__cquorum (gpp : loc) (n : u64) :
+    {{{ own_backup_gpreparer_nrps gpp }}}
+      BackupGroupPreparer__cquorum #gpp #n
+    {{{ RET #(bool_decide (size rids_all / 2 < uint.Z n)); 
+        own_backup_gpreparer_nrps gpp
+    }}}.
+  Proof.
+    iIntros (Φ) "Hgpp HΦ".
+    wp_rec.
+
+    (*@ func (gpp *BackupGroupPreparer) cquorum(n uint64) bool {                @*)
+    (*@     return quorum.ClassicQuorum(gpp.nrps) <= n                          @*)
+    (*@ }                                                                       @*)
+    iNamed "Hgpp".
+    wp_loadField.
+    wp_apply wp_ClassicQuorum.
+    iIntros (x Hx).
+    wp_pures.
+    case_bool_decide as Hc1.
+    { case_bool_decide as Hc2; last word.
+      iApply "HΦ". by iFrame "∗ %".
+    }
+    { case_bool_decide as Hc2; first word.
+      iApply "HΦ". by iFrame "∗ %".
+    }
+  Qed.
+
+  Theorem wp_BackupGroupPreparer__hcquorum (gpp : loc) (n : u64) :
+    {{{ own_backup_gpreparer_nrps gpp }}}
+      BackupGroupPreparer__hcquorum #gpp #n
+    {{{ RET #(bool_decide (size rids_all / 4 + 1 ≤ uint.Z n));
+        own_backup_gpreparer_nrps gpp
+    }}}.
+  Proof.
+    iIntros (Φ) "Hgpp HΦ".
+    wp_rec.
+
+    (*@ func (gpp *BackupGroupPreparer) hcquorum(n uint64) bool {               @*)
+    (*@     return quorum.Half(quorum.ClassicQuorum(gpp.nrps)) <= n             @*)
+    (*@ }                                                                       @*)
+    iNamed "Hgpp".
+    wp_loadField.
+    wp_apply wp_ClassicQuorum.
+    iIntros (x Hx).
+    wp_apply wp_Half.
+    { clear -Hx. word. }
+    iIntros (y Hy).
+    wp_pures.
+    case_bool_decide as Hc1.
+    { case_bool_decide as Hc2; last first.
+      { exfalso. clear -Hnrps Hx Hy Hc1 Hc2. word. }
+      iApply "HΦ". by iFrame "∗ %".
+    }
+    { case_bool_decide as Hc2.
+      { exfalso. clear -Hnrps Hx Hy Hc1 Hc2. word. }
+      iApply "HΦ". by iFrame "∗ %".
+    }
+  Qed.
+
+  Theorem wp_BackupGroupPreparer__latestProposal (gpp : loc) pps rk ts cid gid γ :
+    pps ≠ ∅ ->
+    {{{ own_backup_gpreparer_pps gpp pps rk ts cid gid γ }}}
+      BackupGroupPreparer__latestProposal #gpp
+    {{{ (p : ppsl), RET (ppsl_to_val p); 
+        own_backup_gpreparer_pps gpp pps rk ts cid gid γ ∗
+        ⌜p ∈ (map_img pps : gset ppsl)⌝ ∧
+        ⌜map_Forall (λ _ x, (uint.nat x.1 ≤ uint.nat p.1)%nat) pps⌝
+    }}}.
+  Proof.
+    (*@ func (gpp *BackupGroupPreparer) latestProposal() tulip.PrepareProposal { @*)
+    (*@     var latest tulip.PrepareProposal                                    @*)
+    (*@                                                                         @*)
+    (*@     for _, pp := range(gpp.pps) {                                       @*)
+    (*@         if latest.Rank < pp.Rank {                                      @*)
+    (*@             latest = pp                                                 @*)
+    (*@         }                                                               @*)
+    (*@     }                                                                   @*)
+    (*@                                                                         @*)
+    (*@     return latest                                                       @*)
+    (*@ }                                                                       @*)
+  Admitted.
+
+  Theorem wp_BackupGroupPreparer__becomePreparing (gpp : loc) phase rk ts gid γ :
+    {{{ own_backup_gpreparer_srespm gpp phase rk ts gid γ ∗
+        own_backup_gpreparer_phase gpp phase
+    }}}
+      BackupGroupPreparer__becomePreparing #gpp
+    {{{ RET #(); 
+        own_backup_gpreparer_srespm gpp BGPPPreparing rk ts gid γ ∗
+        own_backup_gpreparer_phase gpp BGPPPreparing
+    }}}.
+  Proof.
+    iIntros (Φ) "[Hsrespm Hphase] HΦ".
+    wp_rec.
+
+    (*@ func (gpp *BackupGroupPreparer) becomePreparing() {                     @*)
+    (*@     gpp.srespm = make(map[uint64]bool)                                  @*)
+    (*@     gpp.phase = BGPP_PREPARING                                          @*)
+    (*@ }                                                                       @*)
+    wp_apply wp_NewMap.
+    iIntros (srespmP) "Hsrespm'".
+    iNamed "Hsrespm". iNamed "Hphase".
+    do 2 wp_storeField.
+    iModIntro.
+    iApply "HΦ".
+    iFrame.
+    iSplit; last done.
+    iSplit; last done.
+    rewrite /prepare_responses dom_empty_L.
+    by iApply big_sepS_empty.
+  Qed.
+
+  Theorem wp_BackupGroupPreparer__becomeUnpreparing (gpp : loc) phase rk ts gid γ :
+    {{{ own_backup_gpreparer_srespm gpp phase rk ts gid γ ∗
+        own_backup_gpreparer_phase gpp phase
+    }}}
+      BackupGroupPreparer__becomeUnpreparing #gpp
+    {{{ RET #(); 
+        own_backup_gpreparer_srespm gpp BGPPUnpreparing rk ts gid γ ∗
+        own_backup_gpreparer_phase gpp BGPPUnpreparing
+    }}}.
+  Proof.
+    iIntros (Φ) "[Hsrespm Hphase] HΦ".
+    wp_rec.
+
+    (*@ func (gpp *BackupGroupPreparer) becomeUnpreparing() {                   @*)
+    (*@     gpp.srespm = make(map[uint64]bool)                                  @*)
+    (*@     gpp.phase = BGPP_UNPREPARING                                        @*)
+    (*@ }                                                                       @*)
+    wp_apply wp_NewMap.
+    iIntros (srespmP) "Hsrespm'".
+    iNamed "Hsrespm". iNamed "Hphase".
+    do 2 wp_storeField.
+    iModIntro.
+    iApply "HΦ".
+    iFrame.
+    iSplit; last done.
+    iSplit; last done.
+    rewrite /prepare_responses dom_empty_L.
+    by iApply big_sepS_empty.
+  Qed.
+
+  Theorem wp_BackupGroupPreparer__countFastProposals
+    (gpp : loc) (b : bool) pps rk ts cid gid γ :
+    {{{ own_backup_gpreparer_pps gpp pps rk ts cid gid γ }}}
+      BackupGroupPreparer__countFastProposals #gpp #b
+    {{{ (n : u64), RET #n;
+        own_backup_gpreparer_pps gpp pps rk ts cid gid γ ∗
+        ⌜uint.nat n = size (filter (λ x, x.2.2 = b) pps)⌝
+    }}}.
+  Proof.
+    iIntros (Φ) "Hpps HΦ".
+    wp_rec.
+
+    (*@ func (gpp *BackupGroupPreparer) countFastProposals(b bool) uint64 {     @*)
+    (*@     var nprep uint64                                                    @*)
+    (*@                                                                         @*)
+    wp_pures.
+    wp_apply wp_ref_of_zero; first by auto.
+    iIntros (nP) "HnP".
+
+    (*@     for _, pp := range(gpp.pps) {                                       @*)
+    (*@         if b == pp.Prepared {                                           @*)
+    (*@             nprep = std.SumAssumeNoOverflow(nprep, 1)                   @*)
+    (*@         }                                                               @*)
+    (*@     }                                                                   @*)
+    (*@                                                                         @*)
+    iNamed "Hpps".
+    wp_loadField.
+    set P := (λ (mx : gmap u64 ppsl),
+                ∃ (n : u64),
+                  "HnP" ∷ nP ↦[uint64T] #n ∗
+                  "%Hn" ∷ ⌜uint.nat n = size (filter (λ x, x.2.2 = b) mx)⌝)%I.
+    wp_apply (wp_MapIter_fold _ _ _ P with "Hpps [$HnP]").
+    { iPureIntro. by rewrite uint_nat_W64_0 map_filter_empty map_size_empty. }
+    { clear Φ.
+      iIntros (mx k v Φ) "!> [HP %Hmk] HΦ".
+      iNamed "HP".
+      wp_pures.
+      destruct Hmk as [Hmk _].
+      case_bool_decide as Hvb; wp_pures.
+      { wp_load.
+        wp_apply wp_SumAssumeNoOverflow.
+        iIntros (Hnoof).
+        wp_store.
+        iApply "HΦ".
+        iFrame.
+        iPureIntro.
+        rewrite uint_nat_word_add_S; last first.
+        { clear -Hnoof. word. }
+        rewrite map_filter_insert_True; last by inv Hvb.
+        rewrite map_size_insert_None; last first.
+        { rewrite map_lookup_filter_None.
+          by left.
+        }
+        by rewrite Hn.
+      }
+      iApply "HΦ".
+      iFrame.
+      iPureIntro.
+      rewrite map_filter_insert_False; last first.
+      { simpl. intros Heq. by rewrite Heq in Hvb. }
+      by rewrite delete_notin.
+    }
+    iIntros "[Hm HP]". iNamed "HP".
+
+    (*@     return nprep                                                        @*)
+    (*@ }                                                                       @*)
+    wp_load.
+    iApply "HΦ".
+    by iFrame "∗ # %".
+  Qed.
+
+  Theorem wp_BackupGroupPreparer__quorumValidated (gpp : loc) ts gid γ :
+    {{{ own_backup_gpreparer_vdm gpp ts gid γ ∗ own_backup_gpreparer_nrps gpp }}}
+      BackupGroupPreparer__quorumValidated #gpp
+    {{{ (vd : bool), RET #vd;
+        own_backup_gpreparer_vdm gpp ts gid γ ∗
+        own_backup_gpreparer_nrps gpp ∗
+        if vd then quorum_validated γ gid ts else True
+    }}}.
+  Proof.
+    iIntros (Φ) "[Hvdm Hnrps] HΦ".
+    wp_rec.
+
+    (*@ func (gpp *BackupGroupPreparer) quorumValidated() bool {                @*)
+    (*@     // Count the number of successful validation.                       @*)
+    (*@     n := uint64(len(gpp.vdm))                                           @*)
+    (*@     // Return if the transaction has been validated on a classic quorum. @*)
+    (*@     return gpp.cquorum(n)                                               @*)
+    (*@ }                                                                       @*)
+    iNamed "Hvdm".
+    wp_loadField.
+    wp_apply (wp_MapLen with "Hvdm").
+    iIntros "[%Hn Hvdm]".
+    wp_apply (wp_BackupGroupPreparer__cquorum with "Hnrps").
+    iIntros "Hnrps".
+    iApply "HΦ".
+    iFrame "∗ # %".
+    case_bool_decide; last done.
+    iExists (dom vdm).
+    iFrame "Hvds".
+    iPureIntro.
+    split; first apply Hvincl.
+    rewrite /cquorum_size size_dom. word.
+  Qed.
+
+  Theorem wp_BackupGroupPreparer__quorumAccepted (gpp : loc) phase rk ts gid γ :
+    (1 < rk)%nat -> 
+    {{{ own_backup_gpreparer_srespm gpp phase rk ts gid γ ∗
+        own_backup_gpreparer_nrps gpp
+    }}}
+      BackupGroupPreparer__quorumAccepted #gpp
+    {{{ (ap : bool), RET #ap;
+        own_backup_gpreparer_srespm gpp phase rk ts gid γ ∗
+        own_backup_gpreparer_nrps gpp ∗
+        if ap
+        then match phase with
+             | BGPPPreparing => quorum_prepared γ gid ts
+             | BGPPUnpreparing => quorum_unprepared γ gid ts
+             | _ => True
+             end
+        else True
+    }}}.
+  Proof.
+    iIntros (Hrk Φ) "[Hsrespm Hnrps] HΦ".
+    wp_rec.
+
+    (*@ func (gpp *BackupGroupPreparer) quorumAccepted() bool {                 @*)
+    (*@     // Count how many replicas have prepared or unprepared, depending on @*)
+    (*@     // @gpp.phase.                                                      @*)
+    (*@     n := uint64(len(gpp.srespm))                                        @*)
+    (*@     return gpp.cquorum(n)                                               @*)
+    (*@ }                                                                       @*)
+    iNamed "Hsrespm".
+    wp_loadField.
+    wp_apply (wp_MapLen with "Hsrespm").
+    iIntros "[%Hn Hsrespm]".
+    wp_apply (wp_BackupGroupPreparer__cquorum with "Hnrps").
+    iIntros "Hnrps".
+    iApply "HΦ".
+    iFrame "∗ # %".
+    case_bool_decide; last done.
+    destruct phase; try done.
+    { iExists rk.
+      rewrite /quorum_pdec_at_rank.
+      case_decide; first word.
+      rewrite /= /quorum_fast_pdec.
+      iExists (dom srespm).
+      iFrame "Hpreps".
+      iPureIntro.
+      split; first apply Hsincl.
+      rewrite /cquorum_size size_dom. word.
+    }
+    { iExists rk.
+      rewrite /quorum_pdec_at_rank.
+      case_decide; first word.
+      rewrite /= /quorum_fast_pdec.
+      iExists (dom srespm).
+      iFrame "Hpreps".
+      iPureIntro.
+      split; first apply Hsincl.
+      rewrite /cquorum_size size_dom. word.
+    }
+  Qed.
+
+  Theorem wp_BackupGroupPreparer__processInquireResult
+    (gpp : loc) (rid : u64) (pp : ppsl) (vd : bool) (pwrsP : loc) (res : rpres)
+    pwrs rk ts cid gid γ :
+    let rkl := uint.nat pp.1 in
+    (1 < rk)%nat ->
+    rid ∈ rids_all ->
+    gid ∈ gids_all ->
+    (if vd then own_map pwrsP DfracDiscarded pwrs else True) -∗
+    inquire_outcome γ gid rid cid ts rk rkl pp.2 vd pwrs res -∗
+    know_tulip_inv γ -∗
+    {{{ own_backup_gpreparer gpp rk ts cid gid γ }}}
+      BackupGroupPreparer__processInquireResult #gpp #rid (ppsl_to_val pp) #vd #pwrsP #(rpres_to_u64 res)
+    {{{ RET #(); own_backup_gpreparer gpp rk ts cid gid γ }}}.
+  Proof.
+    iIntros (rkl Hrk Hrid Hgid) "#Hm #Hinq #Hinv".
+    iIntros (Φ) "!> Hgpp HΦ".
+    wp_rec.
+
+    (*@ func (gpp *BackupGroupPreparer) processInquireResult(rid uint64, pp tulip.PrepareProposal, vd bool, pwrs tulip.KVMap, res uint64) { @*)
+    (*@     // Result is ready or another backup coordinator has become live.   @*)
+    (*@     if gpp.tryResign(res) {                                             @*)
+    (*@         return                                                          @*)
+    (*@     }                                                                   @*)
+    (*@                                                                         @*)
+    iNamed "Hgpp".
+    wp_pures.
+    wp_apply (wp_BackupGroupPreparer__tryResign with "[] Hgpp").
+    { by destruct res. }
+    iIntros (resigned phase') "(Hgpp & %Hres & %Hresigned)".
+    clear phase. rename phase' into phase.
+    destruct resigned; wp_pures.
+    { iApply "HΦ". by iFrame. }
+
+    (*@     // Skip since the coordinator is already in the second phase.       @*)
+    (*@     if gpp.in(BGPP_PREPARING) || gpp.in(BGPP_UNPREPARING) {             @*)
+    (*@         return                                                          @*)
+    (*@     }                                                                   @*)
+    (*@                                                                         @*)
+    wp_apply (wp_BackupGroupPreparer__in _ BGPPPreparing with "Hgpp").
+    iIntros "Hgpp".
+    destruct (bool_decide (phase = BGPPPreparing)) eqn:Hpreparing; wp_pures.
+    { iApply "HΦ". by iFrame. }
+    wp_apply (wp_BackupGroupPreparer__in _ BGPPUnpreparing with "Hgpp").
+    iIntros "Hgpp".
+    destruct (bool_decide (phase = BGPPUnpreparing)) eqn:Hunpreparing; wp_pures.
+    { iApply "HΦ". by iFrame. }
+    rewrite bool_decide_eq_false in Hpreparing.
+    rewrite bool_decide_eq_false in Hunpreparing.
+
+    (*@     // Record prepare prososal and validation result.                   @*)
+    (*@     gpp.collectProposal(rid, pp)                                        @*)
+    (*@     gpp.tryValidate(rid, vd, pwrs)                                      @*)
+    (*@                                                                         @*)
+    (* Prove the only possible res here is [ReplicaOK]. *)
+    destruct res; try done. simpl.
+    iNamed "Hinq". iNamed "Hgpp".
+    wp_apply (wp_BackupGroupPreparer__collectProposal_weak with "Hvote Hlb Hpps").
+    { apply Hrid. }
+    clear pps.
+    iIntros (pps) "Hpps".
+    wp_pures.
+    wp_apply (wp_BackupGroupPreparer__tryValidate with "Hm Hsafepwrs Hvd [$Hpwrs $Hvdm]").
+    { apply Hrid. }
+    iIntros "[Hpwrs Hvdm]".
+    wp_pures.
+
+    (*@     // No decision should be made without a classic quorum of prepare proposals. @*)
+    (*@     n := gpp.countProposals()                                           @*)
+    (*@     if !gpp.cquorum(n) {                                                @*)
+    (*@         return                                                          @*)
+    (*@     }                                                                   @*)
+    (*@                                                                         @*)
+    wp_apply (wp_BackupGroupPreparer__countProposals with "Hpps").
+    iIntros (n) "[Hpps %Hn]".
+    wp_apply (wp_BackupGroupPreparer__cquorum with "Hnrps").
+    iIntros "Hnrps".
+    set c := (bool_decide _).
+    destruct c eqn:Hquorumpsl; wp_pures; last first.
+    { iApply "HΦ". by iFrame "∗ # %". }
+    subst c.
+
+    (* Prepare for making [exclusive_proposal]; we didn't create it explicitly
+    here since we won't always make a proposal here (when going to the
+    VALIDATING state). *)
+    iAssert (quorum_voted γ gid ts rk cid)%I as (ridsvt) "[#Hbkvotes %Hcq]".
+    { iNamed "Hpps".
+      iExists (dom pps).
+      iFrame "Hvotes".
+      iPureIntro.
+      split; first apply Hdompps.
+      clear -Hn Hquorumpsl.
+      rewrite bool_decide_eq_true in Hquorumpsl.
+      rewrite -size_dom in Hn.
+      rewrite /cquorum_size -Hn. lia.
+    }
+    iAssert (own_replica_backup_token γ cid.1 cid.2 ts rk gid)%I
+      with "[Htoken]" as "Htoken".
+    { by destruct phase. }
+
+    (*@     // Compute the latest prepare proposal.                             @*)
+    (*@     latest := gpp.latestProposal()                                      @*)
+    (*@                                                                         @*)
+    wp_apply (wp_BackupGroupPreparer__latestProposal with "Hpps").
+    { rewrite -map_size_non_empty_iff.
+      rewrite bool_decide_eq_true in Hquorumpsl.
+      clear -Hn Hquorumpsl. word.
+    }
+    iIntros (p) "(Hpps & %Hinpps & %Hgeall)".
+    wp_pures.
+
+    (*@     if latest.Rank != 0 {                                               @*)
+    (*@                                                                         @*)
+    set c := (bool_decide _).
+    destruct c eqn:Hnz; wp_pures; last first.
+    { (* First we prove safety of this proposal. *)
+      iAssert (safe_proposal γ gid ts rk p.2)%I as "#Hsafepsl".
+      { iNamed "Hpps".
+        iExists blts.
+        apply elem_of_map_img_1 in Hinpps as [i Hp].
+        rewrite map_Forall2_forall in Hblts.
+        destruct Hblts as [Hblts Hdom].
+        rewrite bool_decide_eq_true in Hquorumpsl.
+        assert (Hlatest : latest_before_quorum rk blts = uint.nat p.1).
+        { (* FIXME: ugly proof and should be a general lemma about [latest_before_quorum]. *)
+          unshelve epose proof (latest_before_quorum_in blts rk _) as Hin.
+          { intros Hempty.
+            rewrite Hempty in Hdom.
+            clear -Hn Hquorumpsl Hdom.
+            apply dom_empty_inv_L in Hdom.
+            rewrite Hdom map_size_empty in Hn.
+            word.
+          }
+          destruct Hin as (j & blt & Hblt & Heq).
+          rewrite -Heq.
+          assert (is_Some (pps !! j)) as [pj Hpj].
+          { by rewrite -elem_of_dom Hdom elem_of_dom. }
+          specialize (Hgeall _ _ Hpj). simpl in Hgeall.
+          specialize (Hblts _ _ _ Hpj Hblt) as Hpjlatest.
+          destruct Hpjlatest as [Hpjlatest _].
+          assert (is_Some (blts !! i)) as [l Hl].
+          { by rewrite -elem_of_dom -Hdom elem_of_dom. }
+          specialize (Hblts _ _ _ Hp Hl) as [Hplatest _].
+          pose proof (latest_before_quorum_ge blts rk) as Hge.
+          specialize (Hge _ _ Hl). simpl in Hge.
+          rewrite -Heq in Hge.
+          specialize (Hlen _ _ Hl) as Hlenl. simpl in Hlenl.
+          specialize (Hlen _ _ Hblt) as Hlenblt. simpl in Hlenblt.
+          rewrite /latest_term -Hlenblt in Hpjlatest.
+          rewrite Hpjlatest.
+          rewrite Hpjlatest in Hge.
+          rewrite /latest_term -Hlenl in Hplatest.
+          rewrite Hplatest in Hge.
+          clear -Hgeall Hge.
+          word.
+        }
+        rewrite Hlatest.
+        iDestruct (big_sepM_lookup with "Hpsl") as "Hpp".
+        { apply Hp. }
+        (* rewrite Hunprep. *)
+        iFrame "#".
+        iPureIntro.
+        split.
+        { rewrite -Hdom.
+          split; first apply Hdompps.
+          clear -Hn Hquorumpsl.
+          rewrite -size_dom in Hn.
+          rewrite /cquorum_size -Hn. lia.
+        }
+        split.
+        { apply (map_Forall_impl _ _ _ Hlen). clear. lia. }
+        { destruct (decide (uint.nat p.1 = 0)%nat) as [Hz | _]; last done.
+          rewrite bool_decide_eq_false in Hnz.
+          clear -Hz Hnz. exfalso.
+          assert (Hp : p.1 = W64 0) by word.
+          by rewrite Hp in Hnz.
+        }
+      }
+
+      (*@         // Unprepare this transaction if its latest slow proposal is @false. @*)
+      (*@         if !latest.Prepared {                                           @*)
+      (*@             gpp.phase = BGPP_UNPREPARING                                @*)
+      (*@             return                                                      @*)
+      (*@         }                                                               @*)
+      (*@                                                                         @*)
+      destruct p.2 eqn:Hunprep; wp_pures; last first.
+      { wp_apply (wp_BackupGroupPreparer__becomeUnpreparing with "[$Hsrespm $Hphase]").
+        iIntros "[Hsrespm Hphase]".
+        wp_pures.
+        iApply "HΦ".
+        iAssert (exclusive_proposal γ gid ts rk)%I with "[Htoken]" as "Hexcl".
+        { rewrite /exclusive_proposal.
+          destruct (decide (rk = 1)%nat); first lia.
+          by iFrame "∗ # %".
+        }
+        iAssert (|={⊤}=> is_group_prepare_proposal γ gid ts rk false)%I with "[Hexcl]" as "> #Hpsl".
+        { iDestruct "Hinv" as (proph) "Hinv".
+          iInv "Hinv" as "> HinvO" "HinvC".
+          iNamed "HinvO".
+          iDestruct (big_sepS_elem_of_acc with "Hgroups") as "[Hgroup HgroupsC]".
+          { apply Hgid. }
+          iMod (group_inv_propose with "Hsafepsl Hexcl Hgroup") as "[Hgroup #Hppsl]".
+          { clear -Hrk. lia. }
+          iDestruct ("HgroupsC" with "Hgroup") as "Hgroups".
+          by iMod ("HinvC" with "[$Htxnsys $Hkeys $Hgroups $Hrgs]") as "_".
+        }
+        by iFrame "∗ #".
+      }
+
+      (*@         // If the latest slow proposal is @true, we further check the   @*)
+      (*@         // availability of partial writes. We might be able to prove it @*)
+      (*@         // without this check by using the fact that a cquorum must have been @*)
+      (*@         // validated in order to prepare in the slow rank, and the fact that @*)
+      (*@         // we've received a cquorum of responses at this point, but the @*)
+      (*@         // reasoning seems pretty tricky. In any case, the check should be valid @*)
+      (*@         // and would eventually passes with some alive cquorum.         @*)
+      (*@         _, ok := gpp.getPwrs()                                          @*)
+      (*@         if !ok {                                                        @*)
+      (*@             return                                                      @*)
+      (*@         }                                                               @*)
+      (*@         gpp.phase = BGPP_PREPARING                                      @*)
+      (*@         return                                                          @*)
+      (*@     }                                                                   @*)
+      (*@                                                                         @*)
+      wp_apply (wp_BackupGroupPreparer__getPwrs with "Hpwrs").
+      iClear "Hm". clear pwrsP.
+      iIntros (pwrsP pwrsok) "[Hpwrs Hm]".
+      wp_pures.
+      destruct pwrsok; wp_pures; last first.
+      { iApply "HΦ". iFrame "∗ #". by destruct phase. }
+      wp_apply (wp_BackupGroupPreparer__becomePreparing with "[$Hsrespm $Hphase]").
+      iIntros "[Hsrespm Hphase]".
+      wp_pures.
+      iApply "HΦ".
+      iAssert (exclusive_proposal γ gid ts rk)%I with "[Htoken]" as "Hexcl".
+      { rewrite /exclusive_proposal.
+        destruct (decide (rk = 1)%nat); first lia.
+        by iFrame "∗ # %".
+      }
+      iAssert (|={⊤}=> is_group_prepare_proposal γ gid ts rk true)%I with "[Hexcl]" as "> #Hpsl".
+      { iDestruct "Hinv" as (proph) "Hinv".
+        iInv "Hinv" as "> HinvO" "HinvC".
+        iNamed "HinvO".
+        iDestruct (big_sepS_elem_of_acc with "Hgroups") as "[Hgroup HgroupsC]".
+        { apply Hgid. }
+        iMod (group_inv_propose with "Hsafepsl Hexcl Hgroup") as "[Hgroup #Hppsl]".
+        { clear -Hrk. lia. }
+        iDestruct ("HgroupsC" with "Hgroup") as "Hgroups".
+        by iMod ("HinvC" with "[$Htxnsys $Hkeys $Hgroups $Hrgs]") as "_".
+      }
+      by iFrame "∗ #".
+    }
+    subst c.
+    rewrite bool_decide_eq_true in Hnz.
+    inv Hnz as [Hz].
+
+    (*@     // All the proposals collected so far are fast. Now we need to decide the @*)
+    (*@     // next step based on how many of them are prepared and unprepared. @*)
+    (*@     nfu := gpp.countFastProposals(false)                                @*)
+    (*@                                                                         @*)
+    wp_apply (wp_BackupGroupPreparer__countFastProposals with "Hpps").
+    iIntros (nfu) "[Hpps %Hnfu]".
+
+    (*@     // Note that using majority (i.e., floor(n / 2) + 1) rather than half (i.e., @*)
+    (*@     // ceiling(n / 2)) as the threshold would lead to liveness issues.  @*)
+    (*@     //                                                                  @*)
+    (*@     // For instance, in a 3-replica setup, using majority means that the @*)
+    (*@     // coordinator can propose UNPREPARED only if it knows there are at least @*)
+    (*@     // two fast unprepares. Consider the following scenario:            @*)
+    (*@     // 1. Replica X fails.                                              @*)
+    (*@     // 2. Txn A validates on replica Y and fails.                       @*)
+    (*@     // 3. Txn B validates on replica Z and fails.                       @*)
+    (*@     // 4. Backup group coordinators of A and B will obtain each one fast @*)
+    (*@     // unprepare (on Z and Y, respetively), so they cannot abort, but also not @*)
+    (*@     // commit since they will not be able to validate on the other replica. @*)
+    (*@     if gpp.hcquorum(nfu) {                                              @*)
+    (*@         // The number of fast unprepares has reached at least half of some @*)
+    (*@         // classic quorum, which means the number of fast prepares must not @*)
+    (*@         // reach a majority in this quorum. This further implies the transaction @*)
+    (*@         // could not have fast prepared, and hence it is safe to unprepare. @*)
+    (*@         //                                                              @*)
+    (*@         // Logical action: Propose.                                     @*)
+    (*@         gpp.phase = BGPP_UNPREPARING                                    @*)
+    (*@         return                                                          @*)
+    (*@     }                                                                   @*)
+    (*@                                                                         @*)
+    wp_apply (wp_BackupGroupPreparer__hcquorum with "Hnrps").
+    iIntros "Hnrps".
+    set c := bool_decide _.
+    destruct c eqn:Huorp; wp_pures.
+    { wp_apply (wp_BackupGroupPreparer__becomeUnpreparing with "[$Hsrespm $Hphase]").
+      iIntros "[Hsrespm Hphase]".
+      wp_pures.
+      iApply "HΦ".
+      iAssert (safe_proposal γ gid ts rk false)%I as "#Hsafepsl".
+      { iNamed "Hpps".
+        iExists blts.
+        apply elem_of_map_img_1 in Hinpps as [i Hp].
+        rewrite map_Forall2_forall in Hblts.
+        destruct Hblts as [Hblts Hdom].
+        rewrite bool_decide_eq_true in Hquorumpsl.
+        assert (Hlatest : latest_before_quorum rk blts = uint.nat p.1).
+        { (* FIXME: ugly proof and should be a general lemma about [latest_before_quorum]. *)
+          unshelve epose proof (latest_before_quorum_in blts rk _) as Hin.
+          { intros Hempty.
+            rewrite Hempty in Hdom.
+            clear -Hn Hquorumpsl Hdom.
+            apply dom_empty_inv_L in Hdom.
+            rewrite Hdom map_size_empty in Hn.
+            word.
+          }
+          destruct Hin as (j & blt & Hblt & Heq).
+          rewrite -Heq.
+          assert (is_Some (pps !! j)) as [pj Hpj].
+          { by rewrite -elem_of_dom Hdom elem_of_dom. }
+          specialize (Hgeall _ _ Hpj). simpl in Hgeall.
+          specialize (Hblts _ _ _ Hpj Hblt) as Hpjlatest.
+          destruct Hpjlatest as [Hpjlatest _].
+          assert (is_Some (blts !! i)) as [l Hl].
+          { by rewrite -elem_of_dom -Hdom elem_of_dom. }
+          specialize (Hblts _ _ _ Hp Hl) as [Hplatest _].
+          pose proof (latest_before_quorum_ge blts rk) as Hge.
+          specialize (Hge _ _ Hl). simpl in Hge.
+          rewrite -Heq in Hge.
+          specialize (Hlen _ _ Hl) as Hlenl. simpl in Hlenl.
+          specialize (Hlen _ _ Hblt) as Hlenblt. simpl in Hlenblt.
+          rewrite /latest_term -Hlenblt in Hpjlatest.
+          rewrite Hpjlatest.
+          rewrite Hpjlatest in Hge.
+          rewrite /latest_term -Hlenl in Hplatest.
+          rewrite Hplatest in Hge.
+          clear -Hgeall Hge.
+          word.
+        }
+        rewrite Hlatest Hz uint_nat_W64_0.
+        iFrame "#".
+        iSplit; first done.
+        iPureIntro.
+        split.
+        { rewrite -Hdom.
+          split; first apply Hdompps.
+          clear -Hn Hquorumpsl.
+          rewrite -size_dom in Hn.
+          rewrite /cquorum_size -Hn. lia.
+        }
+        split.
+        { apply (map_Forall_impl _ _ _ Hlen). clear. lia. }
+        { destruct (decide (O = O)); last done.
+          rewrite bool_decide_eq_true in Huorp.
+          rewrite /nfast.
+          replace (size (filter _ _)) with (uint.nat nfu).
+          { clear -Huorp. lia. }
+          rewrite Hnfu /accepted_in.
+          apply map_Forall2_size_filter.
+          simpl.
+          rewrite map_Forall2_forall.
+          split; last apply Hdom.
+          intros ridx px lx Hpx Hlx.
+          specialize (Hblts _ _ _ Hpx Hlx).
+          destruct Hblts as [Hpx1 Hpx2].
+          pose proof (latest_before_quorum_ge blts rk) as Hallz.
+          rewrite Hlatest Hz uint_nat_W64_0 in Hallz.
+          specialize (Hallz _ _ Hlx). simpl in Hallz.
+          specialize (Hlen _ _ Hlx). simpl in Hlen.
+          rewrite /latest_term -Hlen in Hpx1.
+          assert (Hpx1z : px.1 = W64 0).
+          { clear -Hallz Hpx1. word. }
+          rewrite Hpx1z uint_nat_W64_0 in Hpx2.
+          rewrite Hpx2.
+          split.
+          { intros Heq. by rewrite Heq. }
+          { intros Heq. by inv Heq. }
+        }
+      }
+      iAssert (exclusive_proposal γ gid ts rk)%I with "[Htoken]" as "Hexcl".
+      { rewrite /exclusive_proposal.
+        destruct (decide (rk = 1)%nat); first lia.
+        by iFrame "∗ # %".
+      }
+      iAssert (|={⊤}=> is_group_prepare_proposal γ gid ts rk false)%I
+        with "[Hexcl]" as "> #Hpsl".
+      { iDestruct "Hinv" as (proph) "Hinv".
+        iInv "Hinv" as "> HinvO" "HinvC".
+        iNamed "HinvO".
+        iDestruct (big_sepS_elem_of_acc with "Hgroups") as "[Hgroup HgroupsC]".
+        { apply Hgid. }
+        iMod (group_inv_propose with "Hsafepsl Hexcl Hgroup") as "[Hgroup #Hppsl]".
+        { clear -Hrk. lia. }
+        iDestruct ("HgroupsC" with "Hgroup") as "Hgroups".
+        by iMod ("HinvC" with "[$Htxnsys $Hkeys $Hgroups $Hrgs]") as "_".
+      }
+      by iFrame "∗ #".
+    }
+
+    (*@     // The check below is a proof artifact. We should be able to deduce safety @*)
+    (*@     // of proposing PREPARE from the fact that the number of fast unprepares @*)
+    (*@     // does not reach half, and the fact that decisions are binary. TODO: remove @*)
+    (*@     // this once that is proven.                                        @*)
+    (*@     nfp := gpp.countFastProposals(true)                                 @*)
+    (*@     if !gpp.hcquorum(nfp) {                                             @*)
+    (*@         return                                                          @*)
+    (*@     }                                                                   @*)
+    (*@                                                                         @*)
+    wp_apply (wp_BackupGroupPreparer__countFastProposals with "Hpps").
+    iIntros (nfp) "[Hpps %Hnfp]".
+    wp_apply (wp_BackupGroupPreparer__hcquorum with "Hnrps").
+    iIntros "Hnrps".
+    set d := bool_decide _.
+    destruct d eqn:Hfp; wp_pures; last first.
+    { iApply "HΦ". iFrame "∗ #". by destruct phase. }
+    iAssert (safe_proposal γ gid ts rk true)%I as "#Hsafepsl".
+    { iNamed "Hpps".
+      iExists blts.
+      apply elem_of_map_img_1 in Hinpps as [i Hp].
+      rewrite map_Forall2_forall in Hblts.
+      destruct Hblts as [Hblts Hdom].
+      rewrite bool_decide_eq_true in Hquorumpsl.
+      assert (Hlatest : latest_before_quorum rk blts = uint.nat p.1).
+      { (* FIXME: ugly proof and should be a general lemma about [latest_before_quorum]. *)
+        unshelve epose proof (latest_before_quorum_in blts rk _) as Hin.
+        { intros Hempty.
+          rewrite Hempty in Hdom.
+          clear -Hn Hquorumpsl Hdom.
+          apply dom_empty_inv_L in Hdom.
+          rewrite Hdom map_size_empty in Hn.
+          word.
+        }
+        destruct Hin as (j & blt & Hblt & Heq).
+        rewrite -Heq.
+        assert (is_Some (pps !! j)) as [pj Hpj].
+        { by rewrite -elem_of_dom Hdom elem_of_dom. }
+        specialize (Hgeall _ _ Hpj). simpl in Hgeall.
+        specialize (Hblts _ _ _ Hpj Hblt) as Hpjlatest.
+        destruct Hpjlatest as [Hpjlatest _].
+        assert (is_Some (blts !! i)) as [l Hl].
+        { by rewrite -elem_of_dom -Hdom elem_of_dom. }
+        specialize (Hblts _ _ _ Hp Hl) as [Hplatest _].
+        pose proof (latest_before_quorum_ge blts rk) as Hge.
+        specialize (Hge _ _ Hl). simpl in Hge.
+        rewrite -Heq in Hge.
+        specialize (Hlen _ _ Hl) as Hlenl. simpl in Hlenl.
+        specialize (Hlen _ _ Hblt) as Hlenblt. simpl in Hlenblt.
+        rewrite /latest_term -Hlenblt in Hpjlatest.
+        rewrite Hpjlatest.
+        rewrite Hpjlatest in Hge.
+        rewrite /latest_term -Hlenl in Hplatest.
+        rewrite Hplatest in Hge.
+        clear -Hgeall Hge.
+        word.
+      }
+      rewrite Hlatest Hz uint_nat_W64_0.
+      iFrame "#".
+      iSplit; first done.
+      iPureIntro.
+      split.
+      { rewrite -Hdom.
+        split; first apply Hdompps.
+        clear -Hn Hquorumpsl.
+        rewrite -size_dom in Hn.
+        rewrite /cquorum_size -Hn. lia.
+      }
+      split.
+      { apply (map_Forall_impl _ _ _ Hlen). clear. lia. }
+      { destruct (decide (O = O)); last done.
+        rewrite bool_decide_eq_true in Hfp.
+        rewrite /nfast.
+        replace (size (filter _ _)) with (uint.nat nfp).
+        { clear -Hfp. lia. }
+        rewrite Hnfp /accepted_in.
+        apply map_Forall2_size_filter.
+        simpl.
+        rewrite map_Forall2_forall.
+        split; last apply Hdom.
+        intros ridx px lx Hpx Hlx.
+        specialize (Hblts _ _ _ Hpx Hlx).
+        destruct Hblts as [Hpx1 Hpx2].
+        pose proof (latest_before_quorum_ge blts rk) as Hallz.
+        rewrite Hlatest Hz uint_nat_W64_0 in Hallz.
+        specialize (Hallz _ _ Hlx). simpl in Hallz.
+        specialize (Hlen _ _ Hlx). simpl in Hlen.
+        rewrite /latest_term -Hlen in Hpx1.
+        assert (Hpx1z : px.1 = W64 0).
+        { clear -Hallz Hpx1. word. }
+        rewrite Hpx1z uint_nat_W64_0 in Hpx2.
+        rewrite Hpx2.
+        split.
+        { intros Heq. by rewrite Heq. }
+        { intros Heq. by inv Heq. }
+      }
+    }
+
+    (*@     // At this point, we know there exists a classic quorum in which the number @*)
+    (*@     // of fast unprepares does not reach half (and hence not a majority), @*)
+    (*@     // meaning the transaction could not have fast unprepared. However, we still @*)
+    (*@     // need to ensure validation on a majority to achieve mutual exclusion. @*)
+    (*@                                                                         @*)
+    (*@     // Move to PREPARING phase if it reaches a majority.                @*)
+    (*@     if gpp.quorumValidated() {                                          @*)
+    (*@         // Logical action: Propose.                                     @*)
+    (*@         gpp.phase = BGPP_PREPARING                                      @*)
+    (*@         return                                                          @*)
+    (*@     }                                                                   @*)
+    (*@                                                                         @*)
+    wp_apply (wp_BackupGroupPreparer__quorumValidated with "[$Hvdm $Hnrps]").
+    iIntros (qv) "(Hvdm & Hnrps & #Hqv)".
+    destruct qv; wp_pures.
+    { wp_apply (wp_BackupGroupPreparer__becomePreparing with "[$Hsrespm $Hphase]").
+      iIntros "[Hsrespm Hphase]".
+      wp_pures.
+      iApply "HΦ".
+      iAssert (exclusive_proposal γ gid ts rk)%I with "[Htoken]" as "Hexcl".
+      { rewrite /exclusive_proposal.
+        destruct (decide (rk = 1)%nat); first lia.
+        by iFrame "∗ # %".
+      }
+      iAssert (|={⊤}=> is_group_prepare_proposal γ gid ts rk true)%I
+        with "[Hexcl]" as "> #Hpsl".
+      { iDestruct "Hinv" as (proph) "Hinv".
+        iInv "Hinv" as "> HinvO" "HinvC".
+        iNamed "HinvO".
+        iDestruct (big_sepS_elem_of_acc with "Hgroups") as "[Hgroup HgroupsC]".
+        { apply Hgid. }
+        iMod (group_inv_propose with "Hsafepsl Hexcl Hgroup") as "[Hgroup #Hppsl]".
+        { clear -Hrk. lia. }
+        iDestruct ("HgroupsC" with "Hgroup") as "Hgroups".
+        by iMod ("HinvC" with "[$Htxnsys $Hkeys $Hgroups $Hrgs]") as "_".
+      }
+      by iFrame "∗ #".
+    }
+
+    (*@     // Cannot proceed to the second phase (i.e., proposing prepares or  @*)
+    (*@     // unprepares). Try to validate on more replicas.                   @*)
+    (*@     gpp.phase = BGPP_VALIDATING                                         @*)
+    (*@ }                                                                       @*)
+    iNamed "Hphase".
+    wp_storeField.
+    iApply "HΦ".
+    iDestruct (own_backup_gpreparer_srespm_non_accepting_phase _ _ BGPPValidating
+                with "Hsrespm") as "Hsrespm".
+    { intros []. }
+    by iFrame "∗ #".
+  Qed.
+
+  Theorem wp_BackupGroupPreparer__processValidateResult
+    (gpp : loc) (rid : u64) (res : rpres) rk ts cid gid γ :
+    (1 < rk)%nat ->
+    rid ∈ rids_all ->
+    gid ∈ gids_all ->
+    validate_outcome γ gid rid ts res -∗
+    know_tulip_inv γ -∗
+    {{{ own_backup_gpreparer gpp rk ts cid gid γ }}}
+      BackupGroupPreparer__processValidateResult #gpp #rid #(rpres_to_u64 res)
+    {{{ RET #(); own_backup_gpreparer gpp rk ts cid gid γ }}}.
+  Proof.
+    iIntros (Hrk Hrid Hgid) "#Hvd #Hinv".
+    iIntros (Φ) "!> Hgpp HΦ".
+    wp_rec.
+
+    (*@ func (gpp *BackupGroupPreparer) processValidateResult(rid uint64, res uint64) { @*)
+    (*@     // Result is ready or another backup coordinator has become live.   @*)
+    (*@     if gpp.tryResign(res) {                                             @*)
+    (*@         return                                                          @*)
+    (*@     }                                                                   @*)
+    (*@                                                                         @*)
+    iNamed "Hgpp".
+    wp_apply (wp_BackupGroupPreparer__tryResign with "[] Hgpp").
+    { by destruct res. }
+    iIntros (resigned phase') "(Hgpp & %Hres & %Hresigned)".
+    clear phase. rename phase' into phase.
+    destruct resigned; wp_pures.
+    { iApply "HΦ". by iFrame. }
+
+    (*@     // Skip since the coordinator is already in the second phase.       @*)
+    (*@     if !gpp.in(BGPP_VALIDATING) {                                       @*)
+    (*@         return                                                          @*)
+    (*@     }                                                                   @*)
+    (*@                                                                         @*)
+    wp_apply (wp_BackupGroupPreparer__in _ BGPPValidating with "Hgpp").
+    iIntros "Hgpp".
+    wp_pures.
+    destruct (bool_decide (phase = BGPPValidating)) eqn:Hvalidating; wp_pures; last first.
+    { iApply "HΦ". by iFrame. }
+
+    (*@     // Validation fails; nothing to record.                             @*)
+    (*@     if res == tulip.REPLICA_FAILED_VALIDATION {                         @*)
+    (*@         return                                                          @*)
+    (*@     }                                                                   @*)
+    (*@                                                                         @*)
+    set c := bool_decide _.
+    destruct c eqn:Hfailed; wp_pures.
+    { iApply "HΦ". by iFrame. }
+
+    (*@     // Record success of validation.                                    @*)
+    (*@     gpp.validate(rid)                                                   @*)
+    (*@                                                                         @*)
+    (* Prove the only possible res here is [ReplicaOK]. *)
+    destruct res; try done. simpl.
+    iNamed "Hgpp".
+    wp_apply (wp_BackupGroupPreparer__validate with "Hvd Hvdm").
+    { apply Hrid. }
+    iIntros "Hvdm".
+    
+    (*@     // To be in the VALIDATING phase, we know the transaction must not have fast @*)
+    (*@     // unprepared (need an invariant to remember this fact established when @*)
+    (*@     // transiting from INQUIRING to VALIDATING in @ProcessInquireResult). @*)
+    (*@                                                                         @*)
+    (*@     // Move to PREPARING phase if it reaches a majority.                @*)
+    (*@     if gpp.quorumValidated() {                                          @*)
+    (*@         gpp.becomePreparing()                                           @*)
+    (*@         return                                                          @*)
+    (*@     }                                                                   @*)
+    (*@ }                                                                       @*)
+    wp_apply (wp_BackupGroupPreparer__quorumValidated with "[$Hvdm $Hnrps]").
+    iIntros (vd) "(Hvdm & Hnrps & #Hqv)".
+    destruct vd; wp_pures.
+    { wp_apply (wp_BackupGroupPreparer__becomePreparing with "[$Hsrespm $Hphase]").
+      iIntros "[Hsrespm Hphase]".
+      wp_pures.
+      rewrite bool_decide_eq_true in Hvalidating. subst phase.
+      simpl.
+      iDestruct "Hsafe" as "[Hsafepsl Hqvoted]".
+      iApply "HΦ".
+      iAssert (exclusive_proposal γ gid ts rk)%I with "[Htoken]" as "Hexcl".
+      { rewrite /exclusive_proposal.
+        destruct (decide (rk = 1)%nat); first lia.
+        rewrite /safe_backup_token.
+        iDestruct "Hqvoted" as (rids_votes) "[#Hvotes %Hvotecq]".
+        by iFrame "∗ # %".
+      }
+      iAssert (|={⊤}=> is_group_prepare_proposal γ gid ts rk true)%I with "[Hexcl]" as "> #Hpsl".
+      { iDestruct "Hinv" as (proph) "Hinv".
+        iInv "Hinv" as "> HinvO" "HinvC".
+        iNamed "HinvO".
+        iDestruct (big_sepS_elem_of_acc with "Hgroups") as "[Hgroup HgroupsC]".
+        { apply Hgid. }
+        iMod (group_inv_propose with "Hsafepsl Hexcl Hgroup") as "[Hgroup #Hppsl]".
+        { clear -Hrk. lia. }
+        iDestruct ("HgroupsC" with "Hgroup") as "Hgroups".
+        by iMod ("HinvC" with "[$Htxnsys $Hkeys $Hgroups $Hrgs]") as "_".
+      }
+      by iFrame "∗ #".
+    }
+    iApply "HΦ".
+    by iFrame "∗ #".
+  Qed.
+
+  Definition is_replica_pdec_at_rank_cond γ phase gid rid ts rk : iProp Σ :=
+    match phase with
+    | BGPPPreparing => is_replica_pdec_at_rank γ gid rid ts rk true
+    | BGPPUnpreparing => is_replica_pdec_at_rank γ gid rid ts rk false
+    | _ => True
+    end.
+
+  #[global]
+  Instance is_replica_pdec_at_rank_cond_persistent γ phase gid rid ts rk :
+    Persistent (is_replica_pdec_at_rank_cond γ phase gid rid ts rk).
+  Proof. destruct phase; apply _. Defined.
+
+  Theorem wp_BackupGroupPreparer__accept (gpp : loc) (rid : u64) phase rk ts gid γ :
+    rid ∈ rids_all ->
+    is_replica_pdec_at_rank_cond γ phase gid rid ts rk -∗
+    {{{ own_backup_gpreparer_srespm gpp phase rk ts gid γ }}}
+      BackupGroupPreparer__accept #gpp #rid
+    {{{ RET #(); own_backup_gpreparer_srespm gpp phase rk ts gid γ }}}.
+  Proof.
+    iIntros (Hrid) "#Hpdec".
+    iIntros (Φ) "!> Hsrespm HΦ".
+    wp_rec.
+
+    (*@ func (gpp *BackupGroupPreparer) accept(rid uint64) {                    @*)
+    (*@     gpp.srespm[rid] = true                                              @*)
+    (*@ }                                                                       @*)
+    iNamed "Hsrespm".
+    wp_loadField.
+    wp_apply (wp_MapInsert with "Hsrespm"); first done.
+    iIntros "Hsrespm".
+    wp_pures.
+    iModIntro.
+    iApply "HΦ".
+    iFrame.
+    iSplit.
+    { rewrite /prepare_responses dom_insert_L.
+      destruct phase; try done.
+      { by iApply big_sepS_insert_2. }
+      { by iApply big_sepS_insert_2. }
+    }
+    rewrite dom_insert_L.
+    iPureIntro.
+    set_solver.
+  Qed.
+
+  Theorem wp_BackupGroupPreparer__processPrepareResult
+    (gpp : loc) (rid : u64) (res : rpres) rk ts cid gid γ :
+    (1 < rk)%nat ->
+    rid ∈ rids_all ->
+    accept_outcome γ gid rid ts rk true res -∗
+    {{{ own_backup_gpreparer gpp rk ts cid gid γ }}}
+      BackupGroupPreparer__processPrepareResult #gpp #rid #(rpres_to_u64 res)
+    {{{ RET #(); own_backup_gpreparer gpp rk ts cid gid γ }}}.
+  Proof.
+    iIntros (Hrk Hrid) "#Hacp".
+    iIntros (Φ) "!> Hgpp HΦ".
+    wp_rec.
+
+    (*@ func (gpp *BackupGroupPreparer) processPrepareResult(rid uint64, res uint64) { @*)
+    (*@     // Result is ready or another backup coordinator has become live.   @*)
+    (*@     if gpp.tryResign(res) {                                             @*)
+    (*@         return                                                          @*)
+    (*@     }                                                                   @*)
+    (*@                                                                         @*)
+    iNamed "Hgpp".
+    wp_pures.
+    wp_apply (wp_BackupGroupPreparer__tryResign with "[] Hgpp").
+    { by destruct res. }
+    iIntros (resigned phase') "(Hgpp & %Hres & %Hresigned)".
+    clear phase. rename phase' into phase.
+    destruct resigned; wp_pures.
+    { iApply "HΦ". by iFrame. }
+
+    (*@     if !gpp.in(BGPP_PREPARING) {                                        @*)
+    (*@         return                                                          @*)
+    (*@     }                                                                   @*)
+    (*@                                                                         @*)
+    wp_apply (wp_BackupGroupPreparer__in _ BGPPPreparing with "Hgpp").
+    iIntros "Hgpp".
+    wp_pures.
+    destruct (bool_decide (phase = BGPPPreparing)) eqn:Hpreparing; wp_pures; last first.
+    { iApply "HΦ". by iFrame. }
+    rewrite bool_decide_eq_true in Hpreparing. subst phase.
+
+    (*@     // Prove that at this point the only possible phase is preparing.   @*)
+    (*@     // Resource: Proposal map at rank 1 is true                         @*)
+    (*@     // Invariant: UNPREPARING => proposal map at rank 1 is false: contradiction @*)
+    (*@     // Invariant: Proposal entry present -> not VALIDATING or INQUIRING @*)
+    (*@                                                                         @*)
+    (*@     // Record success of preparing the replica.                         @*)
+    (*@     gpp.accept(rid)                                                     @*)
+    (*@                                                                         @*)
+    (* Prove the only possible res here is [ReplicaOK]. *)
+    destruct res; try done. simpl.
+    iNamed "Hgpp". simpl.
+    wp_apply (wp_BackupGroupPreparer__accept with "[Hacp] Hsrespm").
+    { apply Hrid. }
+    { done. }
+    iIntros "Hsrespm".
+
+    (*@     // A necessary condition to move to the PREPARED phase: validated on some @*)
+    (*@     // classic quorum. TODO: We should be able to remove this check with the @*)
+    (*@     // safe-propose invariant.                                          @*)
+    (*@     if !gpp.quorumValidated() {                                         @*)
+    (*@         return                                                          @*)
+    (*@     }                                                                   @*)
+    (*@                                                                         @*)
+    wp_apply (wp_BackupGroupPreparer__quorumValidated with "[$Hvdm $Hnrps]").
+    iIntros (vd) "(Hvdm & Hnrps & #Hqv)".
+    wp_pures.
+    destruct vd; wp_pures; last first.
+    { iApply "HΦ". by iFrame "∗ #". }
+
+    (*@     // Move to the PREPARED phase if receiving a classic quorum of positive @*)
+    (*@     // prepare responses.                                               @*)
+    (*@     if gpp.quorumAccepted() {                                           @*)
+    (*@         gpp.phase = BGPP_PREPARED                                       @*)
+    (*@     }                                                                   @*)
+    (*@ }                                                                       @*)
+    wp_apply (wp_BackupGroupPreparer__quorumAccepted with "[$Hsrespm $Hnrps]").
+    { apply Hrk. }
+    iIntros (ap) "(Hsrespm & Hnrps & #Hqp)".
+    destruct ap; wp_pures.
+    { iNamed "Hphase".
+      wp_storeField.
+      iApply "HΦ".
+      iDestruct (own_backup_gpreparer_srespm_non_accepting_phase _ _ BGPPPrepared
+                  with "Hsrespm") as "Hsrespm".
+      { intros []. }
+      by iFrame "∗ #".
+    }
+    iApply "HΦ".
+    by iFrame "∗ #".
+  Qed.
+
+  Theorem wp_BackupGroupPreparer__processUnprepareResult
+    (gpp : loc) (rid : u64) (res : rpres) rk ts cid gid γ :
+    (1 < rk)%nat ->
+    rid ∈ rids_all ->
+    accept_outcome γ gid rid ts rk false res -∗
+    {{{ own_backup_gpreparer gpp rk ts cid gid γ }}}
+      BackupGroupPreparer__processUnprepareResult #gpp #rid #(rpres_to_u64 res)
+    {{{ RET #(); own_backup_gpreparer gpp rk ts cid gid γ }}}.
+  Proof.
+    iIntros (Hrk Hrid) "#Hacp".
+    iIntros (Φ) "!> Hgpp HΦ".
+    wp_rec.
+
+    (*@ func (gpp *BackupGroupPreparer) processUnprepareResult(rid uint64, res uint64) { @*)
+    (*@     // Result is ready or another backup coordinator has become live.   @*)
+    (*@     if gpp.tryResign(res) {                                             @*)
+    (*@         return                                                          @*)
+    (*@     }                                                                   @*)
+    (*@                                                                         @*)
+    iNamed "Hgpp".
+    wp_pures.
+    wp_apply (wp_BackupGroupPreparer__tryResign with "[] Hgpp").
+    { by destruct res. }
+    iIntros (resigned phase') "(Hgpp & %Hres & %Hresigned)".
+    clear phase. rename phase' into phase.
+    destruct resigned; wp_pures.
+    { iApply "HΦ". by iFrame. }
+
+    (*@     if !gpp.in(BGPP_UNPREPARING) {                                      @*)
+    (*@         return                                                          @*)
+    (*@     }                                                                   @*)
+    (*@                                                                         @*)
+    wp_apply (wp_BackupGroupPreparer__in _ BGPPUnpreparing with "Hgpp").
+    iIntros "Hgpp".
+    wp_pures.
+    destruct (bool_decide (phase = BGPPUnpreparing)) eqn:Hunpreparing; wp_pures; last first.
+    { iApply "HΦ". by iFrame. }
+    rewrite bool_decide_eq_true in Hunpreparing. subst phase.
+
+    (*@     // Record success of unpreparing the replica.                       @*)
+    (*@     gpp.accept(rid)                                                     @*)
+    (*@                                                                         @*)
+    (* Prove the only possible res here is [ReplicaOK]. *)
+    destruct res; try done. simpl.
+    iNamed "Hgpp". simpl.
+    wp_apply (wp_BackupGroupPreparer__accept with "[Hacp] Hsrespm").
+    { apply Hrid. }
+    { done. }
+    iIntros "Hsrespm".
+
+    (*@     // Move to the ABORTED phase if obtaining a classic quorum of positive @*)
+    (*@     // unprepare responses.                                             @*)
+    (*@     if gpp.quorumAccepted() {                                           @*)
+    (*@         gpp.phase = BGPP_ABORTED                                        @*)
+    (*@     }                                                                   @*)
+    (*@ }                                                                       @*)
+    wp_apply (wp_BackupGroupPreparer__quorumAccepted with "[$Hsrespm $Hnrps]").
+    { apply Hrk. }
+    iIntros (ap) "(Hsrespm & Hnrps & #Hqp)".
+    destruct ap; wp_pures.
+    { iNamed "Hphase".
+      wp_storeField.
+      iApply "HΦ".
+      iDestruct (own_backup_gpreparer_srespm_non_accepting_phase _ _ BGPPAborted
+                  with "Hsrespm") as "Hsrespm".
+      { intros []. }
+      by iFrame "∗ #".
+    }
+    iApply "HΦ".
+    by iFrame "∗ #".
+  Qed.
+
+  Theorem wp_BackupGroupPreparer__stop (gpp : loc) phase :
+    {{{ own_backup_gpreparer_phase gpp phase }}}
+      BackupGroupPreparer__stop #gpp
+    {{{ RET #(); own_backup_gpreparer_phase gpp BGPPStopped }}}.
+  Proof.
+    iIntros (Φ) "Hphase HΦ".
+    wp_rec.
+
+    (*@ func (gpp *BackupGroupPreparer) stop()  {                               @*)
+    (*@     gpp.phase = BGPP_STOPPED                                            @*)
+    (*@ }                                                                       @*)
+    iNamed "Hphase".
+    wp_storeField.
+    iApply "HΦ".
+    by iFrame.
+  Qed.
+
+  Theorem wp_BackupGroupPreparer__processFinalizationResult
+    (gpp : loc) (res : rpres) rk ts cid gid γ :
+    {{{ own_backup_gpreparer gpp rk ts cid gid γ }}}
+      BackupGroupPreparer__processFinalizationResult #gpp #(rpres_to_u64 res)
+    {{{ RET #(); own_backup_gpreparer gpp rk ts cid gid γ }}}.
+  Proof.
+    iIntros (Φ) "Hgpp HΦ".
+    wp_rec.
+
+    (*@ func (gpp *BackupGroupPreparer) processFinalizationResult(res uint64) { @*)
+    (*@     if res == tulip.REPLICA_WRONG_LEADER {                              @*)
+    (*@         return                                                          @*)
+    (*@     }                                                                   @*)
+    (*@     gpp.stop()                                                          @*)
+    (*@ }                                                                       @*)
+    wp_pures.
+    case_bool_decide; wp_pures.
+    { by iApply "HΦ". }
+    do 2 iNamed "Hgpp".
+    wp_apply (wp_BackupGroupPreparer__stop with "Hphase").
+    iIntros "Hphase".
+    wp_pures.
+    iModIntro.
+    iApply "HΦ".
+    iFrame "∗ #". simpl.
+    iSplit.
+    { iApply (own_backup_gpreparer_srespm_non_accepting_phase with "Hsrespm").
+      intros [].
+    }
+    done.
+  Qed.
+
+  Theorem wp_BackupGroupPreparer__processQueryResult
+    (gpp : loc) (rid : u64) (res : rpres) rk ts cid gid γ :
+    query_outcome γ ts res -∗
+    {{{ own_backup_gpreparer gpp rk ts cid gid γ }}}
+      BackupGroupPreparer__processQueryResult #gpp #rid #(rpres_to_u64 res)
+    {{{ RET #(); own_backup_gpreparer gpp rk ts cid gid γ }}}.
+  Proof.
+    iIntros "#Hquery" (Φ) "!> Hgpp HΦ".
+    wp_rec.
+
+    (*@ func (gpp *BackupGroupPreparer) processQueryResult(rid uint64, res uint64) { @*)
+    (*@     gpp.tryResign(res)                                                  @*)
+    (*@ }                                                                       @*)
+    iNamed "Hgpp".
+    wp_apply (wp_BackupGroupPreparer__tryResign with "[] Hgpp").
+    { by destruct res. }
+    iIntros (resigned phase') "(Hgpp & %Hres & %Hresigned)".
+    wp_pures.
+    iApply "HΦ".
+    by iFrame.
   Qed.
 
 End bgpreparer.
@@ -547,7 +2214,7 @@ Section bgcoord.
     iIntros "[Hlocked Hgcoord]".
     iNamed "Hgcoord". iNamed "Hgpp".
     wp_loadField.
-    wp_apply (wp_BackupGroupPreparer__getPwrs with "Hgpp").
+    wp_apply (wp_BackupGroupPreparer__getPwrs_external with "Hgpp").
     iIntros (pwrsP pwrsok) "[Hgpp #Hpwrs]".
     wp_loadField.
     wp_apply (wp_Mutex__Unlock with "[-HΦ]").
@@ -821,8 +2488,8 @@ Section bgcoord.
     (*@     }                                                                   @*)
     (*@                                                                         @*)
     set P := (λ (cont : bool), ∃ (phase' : bgppphase) (gppP' : loc),
-                 "HgppP"   ∷ gcoord ↦[BackupGroupCoordinator::"gpp"] #gppP' ∗
-                 "Hgpp"    ∷ own_backup_gpreparer_with_phase gppP' phase' rk ts gid γ ∗
+                 "HgppP"   ∷ gcoord ↦[BackupGroupCoordinator :: "gpp"] #gppP' ∗
+                 "Hgpp"    ∷ own_backup_gpreparer_with_phase gppP' phase' rk ts cid gid γ ∗
                  "Hcomm"   ∷ own_backup_gcoord_comm gcoord addrm gid γ ∗
                  "Hlocked" ∷ locked #muP ∗
                  "%Hready" ∷ ⌜if cont then True else bgpp_ready phase'⌝)%I.
